@prefix rdf:    <http://www.w3.org/1999/02/22-rdf-syntax-ns#> .
@prefix rdfs:   <http://www.w3.org/2000/01/rdf-schema#> .
@prefix xsd:    <http://www.w3.org/2001/XMLSchema#> .
@prefix :       <http://www.example.com/cristin-ontology#> .

#Info about rdfs types
#https://www.w3.org/TR/rdf-schema/#ch_resource

:CristinClass
    a            rdfs:Class ;
    rdfs:label   "CristinClass" ;
    rdfs:comment "Any class that represent an entity or collection of values in Cristin" .

:Result
    a               :CristinClass ;
    rdfs:subClassOf :CristinClass ;
    rdfs:comment    "The equivalent of an NVA Resource in Cristin. An database entry as being exported especially for importing in NVA" .

:cristinfield
    a            rdf:Property ;
    rdfs:comment "Any property of any Cristin class" ;
    rdfs:domain  :CristinClass ;
    rdfs:range   rdfs:Class .

:mapstonvafield
    a            rdf:Property ;
    rdfs:comment """ A short description on how we save this information to NVA.""" ;
    rdfs:range   xsd:string ;
    rdfs:domain  :cristinfield .

:currently_ignored
    a            rdf:Property ;
    rdfs:comment """Indicates whether at present we are using this field or not. Used for keeping track of the fields that
            we are mapping to NVA and the ones that we are not. It does not mean that the ignored fields will not be included,
            it mean that currently we have not included them""" ;
    rdfs:range   xsd:boolean ;
    rdfs:domain  :cristinfield .


:should_ignore
    a            rdf:Property ;
    rdfs:comment """
    Indicates that according to the common understanding the field should be ignored in the final mapping of the Cristin data.
    Preferably the field should not be included in the Cristin exports
    """ ;
    rdfs:range   xsd:boolean ;
    rdfs:domain  :cristinfield .


:PublicationStatus
    a :CristinClass .

:Published
    a               rdfs:Class ;
    rdfs:label      "PUBLISERT" ;
    rdfs:subClassOf :PublicationStatus .

:InPress
    a               rdfs:Class ;
    rdfs:label      "IN_PRESS" ;
    rdfs:subClassOf :PublicationStatus .

:TestPublicationStatus
    a               rdfs:Class ;
    rdfs:label      "TEST" ;
    rdfs:subClassOf :PublicationStatus .

:VARBEID_SPRAK_Class
    a               rdfs:Class ;
    rdfs:subClassOf :CristinClass ;
    rdfs:comment    """
    The structure defining the VARBEID_SPRAK property.
    A language that this work has been published in, the respective title, and the respective abstract
    and an indication whether it is the original language or a translation.
    The Cristin Result can have multiple varbeid_sprak objects.""" .

:VARBEID_PERSON_Class
    a            rdfs:Class ;
    rdfs:comment """
    The structure of the VARARBEID_PERSON entry. It contains user submitted information about the status of the contributor
    at the time the Result was registered in Cristin. Some of the information can be  provided by the user manually in order to reflect the
    user's name at the time the manuscript/publication was submitted to the publisher (e.g. Elsevier).
    """ .


:VARBEID_PERSON_STED_Class
    a               rdfs:Class ;
    rdfs:subClassOf :CristinClass ;
    rdfs:comment    """
    The structure of the VARBEID_PERSON_STED entry.
    The entry contains information about the contributor's institutional affiliation represented in the result entity
     at the time of publication, as well as the current instance of that institution, should it have evolved over time.
    """ .


:VARBEID_PERSON_STED_ROLLE_Class
    a               rdfs:Class ;
    rdfs:subClassOf :CristinClass ;
    rdfs:comment    """
     The structure of VARBEID_PERSON_STED_ROLLE. It contains information about the role of
    the contributor in this publication. One contributor can have many different contribution roles from the same or different institutions.
    Example:
    Contributor C has contributed as "EDITOR" affiliated with InstA for publication P
    and they have contributed as "ILLUSTRATOR" affiliated with InstB for the same publication.
    """ .

:TYPE_MEDIEBIDRAG_Class
    a               rdfs:Class ;
    rdfs:subClassOf :CristinClass ;
    rdfs:comment    """
    The structure of TYPE_MEDIEBIDRAG. It contains information for publications in one of the following media.
    Newspaper(AVIS),
    TV ,
    Internet (INTERNETT)
    Radio(RADIO)
    Journal (TIDSSKRIFT)
    FAGBLAD.
    The  categories of publications are Documentary(DOKUMENTAR), Interview (INTERVJU), PROGDELTAGELSE, PROGLEDELSE
    """ .

:PRESENTASJON_VARBEID_Class
    a               rdfs:Class ;
    rdfs:subClassOf :CristinClass ;
    rdfs:comment    """
    Reference to a project when :presentasjonstypekode is equal to :PRESENTASJONSTYPEKODE_PROSJEKT. More information in the
    description of the field :presentasjonstypekode.
    """ .

:PRESENTASJONSTYPEKODE_VALUES_Class
    a            rdfs:Class ;
    rdfs:comment """Values for the enum of PRESENTASJONSTYPEKODE """ .


:PRESENTASJONSTYPEKODE_PERSON
    a               rdfs:Class ;
    rdfs:label      "PERSON" ;
    rdfs:comment    "Indicates reference to a Cristin person profile, which in turn refers to a Cristin person id." ;
    rdfs:subClassOf :PRESENTASJONSTYPEKODE_VALUES_Class .

:PRESENTASJONSTYPEKODE_GRUPPE
    a               rdfs:Class ;
    rdfs:label      "GRUPPE" ;
    rdfs:comment    "UNKNOWN MEANING. When :presentasjonstypekode has this value, the reference is not a project." ;
    rdfs:subClassOf :PRESENTASJONSTYPEKODE_VALUES_Class .


:PRESENTASJONSTYPEKODE_PROSJEKT
    a               rdfs:Class ;
    rdfs:label      "PROSJEKT" ;
    rdfs:subClassOf :PRESENTASJONSTYPEKODE_VALUES_Class .

:FINANSIERING_VARBEID_Class
    a            :CristinClass ;
    rdfs:comment """
    The structure of FINANSIERING_VARBEID. Information about funding (research grants) underlying this result.
    This field resolves only grants specifically attached to this result.

    Note that funding / research grants attached to Cristin projects claiming this result must be resolved through the
    project at https://api.cristin.no/v2/projects/<project_id>

    Owing to the number of funding bodies, there is no uniform way to dereference grants externally.
    """ .

:TYPE_BOK_RAPPORT_DEL_Class
    a               rdfs:Class ;
    rdfs:subClassOf :CristinClass ;
    rdfs:comment    """
    Indicates that the respective  publication is a part of book or report.
    The field TYPE_BOK_RAPPORT_DEL.inngar_i contains the reference to the parent Cristin entry about that book or report.
    The secondary categories that have such a field are
    	ANNET
	    INNLEDNING
	    FORORD
	    OVERSETTELSE_KAP
	    KAPITTEL
	    LEKSIKAL_INNF
        POPVIT_KAPITTEL
	    FAGLIG_KAPITTEL
    """ ;
    rdfs:domain     :Result .


:PRESENTASJONSTYPEKODE_ENHET
    a               rdfs:Class ;
    rdfs:label      "ENHET" ;
    rdfs:comment    "UNKNOWN MEANING. When :presentasjonstypekode has this value, the reference is not a project." ;
    rdfs:subClassOf :PRESENTASJONSTYPEKODE_VALUES_Class .

:PRESENTASJONSTYPEKODE_SENTER
    a               rdfs:Class ;
    rdfs:label      "SENTER" ;
    rdfs:comment    "UNKNOWN MEANING. When :presentasjonstypekode has this value, the reference is not a project." ;
    rdfs:subClassOf :PRESENTASJONSTYPEKODE_VALUES_Class .

:VARBEID_KILDE_Class
    a               rdfs:Class ;
    rdfs:subClassOf :CristinClass ;
    rdfs:comment    """
         When this entry is populated, the respective entry is imported from another source.
         E.g. FORSKDOK or SCOPUS a predecessor of Cristin
         """ .

:VITENSKAPELIGARBEID_LOKAL_Class
    a               rdfs:Class ;
    rdfs:subClassOf :CristinClass ;
    rdfs:comment    """
        This field contains metadata relevant for NVI reporting, one set per contributing institution that is also part of the NVI process.
        The contained metadata are related to the users that created/updated the entry for the NVI report. For example "brukernavn_opprettet"
        refers to the superuser that created the NVI entry and not the user that created the Cristin entry.
    """ .


:VARBEID_VDISIPLIN_Class
    a            :CristinClass ;
    rdfs:comment """
            This field contains metadata about the scientific discipline to which the publication belongs.
            The data is structured hierarchical with gradually more fine grained discipline specifications
            """ .

:TYPE_BOK_RAPPORT_Class
    a               rdfs:Class ;
    rdfs:subClassOf :CristinClass ;
    rdfs:comment    """
         The respective object contains metadata about a book.
         The respective field (TYPE_BOK_RAPPORT) has a value only if the varbeidhovedkatkode has one of the following values:
         OVERSETTELSESARB
         RAPPORT
         BOK.
         The Cristin secondary categories (varbeidunderkatkode)
         that are expected to have such an entry are the following:
         ANTOLOGI
         DRGRADAVH
         FAGBOK
         FORSKERLINJEOPPG
         HOVEDFAGSOPPGAVE
         KOMMENTARUTG
         KOMPENDIUM
         LEKSIKON
         LISENSIATAVH
         LÃ†REBOK
         MAGISTERAVH
         MASTERGRADSOPPG
         MONOGRAFI
         OPPSLAGSVERK
         OVERSETTELSE_BOK
         POPVIT_BOK
         RAPPORT
         UTSTILLINGSKAT
         """ .

:FAGFELT_Class
    a               rdfs:Class ;
    rdfs:subClassOf :CristinClass ;
    rdfs:comment    """A reference to the NSD scientific field in which the book/chapter is published. All NSD fields are listed here: https://npi.nsd.no/fagfeltoversikt/
    """ ;
    rdfs:domain     :TYPE_BOK_RAPPORT_Class, :TYPE_BOK_RAPPORT_DEL_Class .

:TYPE_TIDSSKRIFTPUBLIKASJON_Class
    a               rdfs:Class ;
    rdfs:subClassOf :CristinClass ;
    rdfs:comment    """
        A type of publication/result published in a journal, typically articles, reviews or editorials.
       """ .

:TIDSSKRIFT_Class
    a               rdfs:Class ;
    rdfs:subClassOf :CristinClass ;
    rdfs:comment    """Metadata about a scientific journal.""" .

:VARBEID_EMNEORD_Class
    a               rdfs:Class ;
    rdfs:subClassOf :CristinClass ;
    rdfs:comment    """A keyword that is relative to a publication.""" .

:VARBEID_HRCS_KLASSIFISERING_Class
    a               rdfs:Class ;
    rdfs:subClassOf :CristinClass ;
    rdfs:comment    """Classification of the publication with respect to the UKCRC Health Research Classification System (HRCS).""" .

:FORLAG_Class
    a               rdfs:Class ;
    rdfs:subClassOf :CristinClass ;
    rdfs:comment    """
    Information about the Publishing House that published a Book or a Report. It is important to note that when a Book belongs to a series,
    then it is possible that a series will have a different publisher than the book. I.e., one publishing house is publishing the series but another
    publishing house is publishing the book belonging to the series.

    """ .

:id
    a               :cristinfield ;
    rdfs:comment    "Identifier of Cristin Result entry." ;
    rdfs:range      xsd:positiveInteger ;
    rdfs:domain     :Result ; .

:arstall
    a               :cristinfield ;
    rdfs:comment    "The year a resource (result) was published." ;
    rdfs:range      xsd:positiveInteger ;
    rdfs:domain     :Result ; .

:dato_opprettet
    a                  :cristinfield ;
    rdfs:comment       """
    When the domain is :Result, it is the date the resource was registered in Cristin or its predecessor.
    When the domain is :VITENSKAPELIGARBEID_LOKAL, it is the date the resource was registered in NVI.
    """ ;
    rdfs:range         xsd:date ;
    rdfs:domain        :Result, :VITENSKAPELIGARBEID_LOKAL_Class ;
    :currently_ignored "true" .


:varbeidhovedkatkode
    a               :cristinfield ;
    rdfs:comment    """
    The general category of the resource. A collection of "varbeidunderkatkode" .

""" ;
    rdfs:range      xsd:string ;
    rdfs:domain     :Result ; .

:varbeidunderkatkode
    a               :cristinfield ;
    rdfs:comment    """
        The more specific category of the resource. No specific range available at the moment.
        Each varbeidunderkatkode belongs to only one varbeidhovedkatkode and therefore the value of this field is enough
        to deduct the exact type of the publication.
        The range of this property is found here:  https://api.cristin.no/v2/results/categories?lang=nb ,  en
        """ ;
    rdfs:range      xsd:string ;
    rdfs:domain     :Result ; .

:eierkode_opprettet
    a            :cristinfield ;
    rdfs:comment """
        eierkode_opprettet and brukernavn_opprettet are the primary key for idenitfying which user created the entry. As a general rule a physical person
        can have many usernames (brukernavn) but only one eierkode. This holds even if a physical person moves from institution to institution
        and/or changes roles. Duplicates that violate this assumption are possible to occur but they are not expected to be the rule.
     """ ;
    rdfs:range   xsd:string ;
    rdfs:domain  :Result .


:brukernavn_opprettet
    a                  :cristinfield ;
    rdfs:comment       """
        When the domain is :Result, eierkode_opprettet and brukernavn_opprettet are the primary key for idenitfying which user created the entry. As a general rule a physical person
        can have many usernames (brukernavn) but only one eierkode. This holds even if a physical person moves from institution to institution
        and/or changes roles. Duplicates that violate this assumption are possible to occur but they are not expected to be the rule.

        When it is :VITENSKAPELIGARBEID_LOKAL_Class it is the user who created the NVI entry."
     """ ;
    rdfs:range         xsd:string ;
    rdfs:domain        :Result, :VITENSKAPELIGARBEID_LOKAL_Class ;
    :currently_ignored "true" .


:eierkode_siste_endring
    a                  :cristinfield ;
    rdfs:comment       "Similar to eierkode_opprettet but it indicates who made the last change." ;
    rdfs:range         xsd:string ;
    rdfs:domain        :Result ;
    :currently_ignored "true" .

:brukernavn_siste_endring
    a                  :cristinfield ;
    rdfs:comment       """
    When the domain is :Result the meaning is similar to brukernavn_opprettet but it indicates who made the last change.
    When the domain is :VITENSKAPELIGARBEID_LOKAL_Class  then it is the username of the user who updated the NVI entry.
     """ ;
    rdfs:range         xsd:string ;
    rdfs:domain        :Result, :VITENSKAPELIGARBEID_LOKAL_Class ;
    :currently_ignored "true" .

:dato_siste_endring
    a                  :cristinfield ;
    rdfs:comment       """
    When the domain is :Result, then the date of the last update of the registration.
    When the domain is :VITENSKAPELIGARBEID_LOKAL_Class then it is date the NVI entry was last updated
        """ ;
    rdfs:range         xsd:date ;
    rdfs:domain        :Result, :VITENSKAPELIGARBEID_LOKAL_Class ;
    :currently_ignored "true" .


:publiseringstatuskode
    a               :cristinfield ;
    rdfs:comment    """
                            The publication status of the referenced publication, i.e. whether the publication status of the publication itself in the publisher (e.g. Elsevier)
                            Possible values are: IN_PRESS", "PUBLISERT" (and "TEST").
                            """ ;
    rdfs:range      :PublicationStatus ;
    rdfs:domain     :Result ;
    :mapstonvafield "status = PUBLISHED (hardcoded)" .

:dato_utgitt
    a                  :cristinfield ;
    rdfs:comment       "Date the resource was published (e.g. through Elsevier or in OpenAccess Journal)." ;
    rdfs:range         xsd:date ;
    rdfs:domain        :Result ;
    :currently_ignored "true" .

:arstall_rapportert
    a                  :cristinfield ;
    rdfs:comment       "Year that the resource was included in an NVI report." ;
    rdfs:range         xsd:positiveInteger ;
    rdfs:domain        :Result ;
    :currently_ignored "true" .

:merknadtekst
    a                  :cristinfield ;
    rdfs:comment       "Free text for super-users to add comments when it comes to NVI approvals." ;
    rdfs:range         xsd:string ;
    rdfs:domain        :Result ;
    :currently_ignored "true" .

:merknadtekst_godkjenning
    a                  :cristinfield ;
    rdfs:comment       "Free text for super-users to add explanations/details on why the publication was approved or rejectedfor NVI reporting." ;
    rdfs:range         xsd:string ;
    rdfs:domain        :Result ;
    :currently_ignored "true" .

:kildekode
    a                  :cristinfield ;
    rdfs:comment       """
    The source (provider) the result was imported from, if any.
    Mostly superseded by the list of import references in table VARBEID_KILDE
    It is a string containing arbitrary codes such as "scopus" "norart", "BIBSYS" etc.
    """ ;
    rdfs:range         xsd:string ;
    rdfs:domain        :Result, :VARBEID_KILDE_Class ;
    :currently_ignored "true" .

:kildepostid
    a                  :cristinfield ;
    rdfs:comment       """
    The id of the record the result was imported from in the source system (e.g. the SCOPUS id if the result was imported from Scopus ) .

See varbeid.kildekode. Mostly superseded by VARBEID_KILDE. It contains only the identifier found in the source system and cannot be
     de-referenced.
    """ ;
    rdfs:range         xsd:string ;
    rdfs:domain        :Result ;
    :currently_ignored "true" .

:kildeid
    a            :cristinfield ;
    rdfs:domain  :VARBEID_KILDE_Class ;
    rdfs:range   xsd:string ;
    rdfs:comment """
        The id of the record from the source it was imported
( e.g SCOPUS or FORSKDOK. Overseeds :kildepostid.
    """ .


:pubidnr
    a                  :cristinfield ;
    rdfs:comment       """
    A reference to the record corresponding to this result in the PIA import database.
    PIA is a database that holds imports from Scopus.
    """ ;
    rdfs:range         xsd:positiveInteger ;
    rdfs:domain        :Result ;
    :currently_ignored "true" .

:VARBEID_SPRAK
    a               :cristinfield ;
    rdfs:comment    """See the description of the range class. """ ;
    rdfs:range      :VARBEID_SPRAK_Class ;
    rdfs:domain     :Result ; .

:sprakkode
    a               :cristinfield ;
    rdfs:comment    """
    When the domain in :VARARBEID_SPRAK it is the language of the title and the abstract included in the entry
    When the domain is :TIDSSKRIFT it is the language used in the journal, this may not be the same as the article contained within.
    The range is ISO 639-1.
    Possibly null or (xx) to represent (n/a)
    """ ;
    rdfs:range      xsd:string ;
    rdfs:domain     :VARBEID_SPRAK_Class, :TIDSSKRIFT_Class ; .

:tittletekst
    a               :cristinfield ;
    rdfs:comment    "The title in the VARARBEID_SPRAK entry. It is supposed to be in the language described by :sprakkode" ;
    rdfs:range      xsd:string ;
    rdfs:domain     :VARBEID_SPRAK_Class ; .


:sammendragtekst
    a               :cristinfield ;
    rdfs:comment    "The abstract in the VARARBEID_SPRAK entry. It is supposed to be in the language described by :sprakkode" ;
    rdfs:range      xsd:string ;
    rdfs:domain     :VARBEID_SPRAK_Class ; .

:status_original
    a                  :cristinfield ;
    rdfs:comment       """
    Indicator of whether the title and the abstract is in the respective VARBEID_SPRAK is in the original language and if so, then they are the original title and abstract.
    Known possible values are 'J' ('true')
        , 'N' (false) and NULL (free to interpretation ) .

""" ;
    rdfs:range         xsd:string ;
    rdfs:domain        :VARBEID_SPRAK_Class ;
    :currently_ignored "false" .

:VITENSKAPELIGARBEID_LOKAL
    a                  :cristinfield ;
    rdfs:comment       "See description of domain class" ;
    rdfs:domain        :Result ;
    rdfs:range         :VITENSKAPELIGARBEID_LOKAL_Class ;
    :currently_ignored "true" .

:VARBEID_PERSON
    a               :cristinfield ;
    rdfs:comment    "See description in range class." ;
    rdfs:range      :VARBEID_PERSON_Class ;
    rdfs:domain     :Result ; .

:personlopenr
    a                  :cristinfield ;
    rdfs:comment       """
    It refers to a person's CristinId.
    When the domain is :VARBEID_PERSON_Class then it is a reference to a contributor.
    When the domain is "PRESENTASJON_VARBEID_Class and  the respective presentasjonstypekode is equal to "PERSON", tt refers to a contributor that has chosen
    to show this publication as one of their "important", "significant" etc publications.
    """ ;
    rdfs:range         xsd:positiveInteger ;
    rdfs:domain        :VARBEID_PERSON_Class, :PRESENTASJON_VARBEID_Class ;
    :currently_ignored false .


:fornavn
    a               :cristinfield ;
    rdfs:comment    """The first/given name of the contributor of the respective result entry.
                        This value is submitted manually by the user, in order to reflect what the user submitted as their first name when they
                        submitted the publication to the publisher
(e.g. Elsevier)
        """ ;
    rdfs:range      xsd:string ;
    rdfs:domain     :VARBEID_PERSON_Class ; .

:etternavn
    a               :cristinfield ;
    rdfs:comment    """
    The surname/family-name of the contributor of the respective result entry
    This value is submitted manually by the user, in order to reflect what the user submitted as their first name when they
        submitted the publication to the publisher ( e.g. Elsevier ) .
""" ;
    rdfs:range      xsd:string ;
    rdfs:domain     :VARBEID_PERSON_Class ; .

:rekkefolgenr
    a               :cristinfield ;
    rdfs:comment    "An integer informing in what place among the other contributers this particular one is to be listed.";
    rdfs:range      :VARBEID_PERSON_Class ;
    rdfs:domain     xsd:positiveInteger ;
    :currently_ignored false.

:VARBEID_PERSON_STED
    a               :cristinfield ;
    rdfs:comment    "See description in range class" ;
    rdfs:range      :VARBEID_PERSON_STED_Class ;
    rdfs:domain     :VARBEID_PERSON_Class ; .


:institusjonsnr
    a               :cristinfield ;
    rdfs:comment    """
    The **current** Cristin institution identifier institution that the contributor of the publication was affiliated with.
    This value may have changed from the time of entry was registered in
Cristin.
   :institusjonsnr
        ,   :avdnr, :undavdnr, and :gruppenr form a unique identifier of the Contributor's affiliation.

    """ ;
    rdfs:range      xsd:positiveInteger ;
    rdfs:domain     :VARBEID_PERSON_STED_Class ; .

:avdnr
    a               :cristinfield ;
    rdfs:comment    """
    The **current** Cristin Department number that the contributor of the publication was affiliated with at the time of creation of the
    registration entry.
    This value may have changed from the time of entry was registered in Cristin.
    See example in the definition of the domain class :VARBEID_PERSON_STED_Class
    """ ;
    rdfs:range      xsd:positiveInteger ;
    rdfs:domain     :VARBEID_PERSON_STED_Class ; .

:undavdnr
    a               :cristinfield ;
    rdfs:comment    """
    The current Sub-department number that the contributor of the publication was affiliated with at the time of creation of the
    registration entry.
    This value may have changed from the time of entry was registered in Cristin.
    See example in the definition of the domain class :VARBEID_PERSON_STED_Class
    """ ;
    rdfs:range      xsd:positiveInteger ;
    rdfs:domain     :VARBEID_PERSON_STED_Class ; .

:gruppenr
    a               :cristinfield ;
    rdfs:comment    """
     The current group number that the contributor of the publication was affiliated with at the time of creation of the registration entry.
     This value may have changed from the time of entry was registered in Cristin.
    """ ;
    rdfs:range      xsd:positiveInteger ;
    rdfs:domain     :VARBEID_PERSON_STED_Class ; .

:stedkode_opprinnelig
    a                  :cristinfield ;
    rdfs:comment       """
    This is a concatenation of :institusjonsnr, :avdnr, :undavdnr and gruppenr and it indicates the original identifier of the
    institution when the Cristin entry was created. This is an immutable value that never changes after its creation.
    """ ;
    rdfs:range         xsd:string ;
    rdfs:domain        :VARBEID_PERSON_STED_Class ;
    :currently_ignored "true" .

:institusjonsnavn_opprinnelig
    a                  :cristinfield ;
    rdfs:comment       "The original name of the institution at the time the Cristin entry was created. Immutable value" ;
    rdfs:range         xsd:string ;
    rdfs:domain        :VARBEID_PERSON_STED_Class ;
    :currently_ignored "true" .

:avdelingsnavn_opprinnelig
    a                  :cristinfield ;
    rdfs:comment       "The original name of the department at the time the Cristin entry was created. Immutable value" ;
    rdfs:range         xsd:string ;
    rdfs:domain        :VARBEID_PERSON_STED_Class ;
    :currently_ignored "true" .

:stednavn_opprinnelig
    a                  :cristinfield ;
    rdfs:comment       """
    The original name of the faculty/group that the Contributor was affiliated with at the time the Cristin entry was created.
    Hierarchically, this is the name of the lowest (most specific) entity that the Contributor is affiliated with.
     """ ;
    rdfs:range         xsd:string ;
    rdfs:domain        :VARBEID_PERSON_STED_Class ;
    :currently_ignored "true" .

:VARBEID_PERSON_STED_ROLLE
    a               :cristinfield ;
    rdfs:comment    "See description in range class" ;
    rdfs:range      :VARBEID_PERSON_STED_ROLLE_Class ;
    rdfs:domain     :VARBEID_PERSON_STED_Class ; .

:rollekode
    a                  :cristinfield ;
    rdfs:comment       """
        The role of the respective Contributor for the respective publication affiliated for this role with the respective institution.
        This entry is immutable and does not change in time.
        """ ;
    rdfs:range         xsd:string ;
    rdfs:domain        :VARBEID_PERSON_STED_ROLLE_Class ;
    :currently_ignored false ;.

:eierkode
    a                  :cristinfield ;
    rdfs:range         xsd:string ;
    rdfs:domain        :VITENSKAPELIGARBEID_LOKAL_Class ;
    rdfs:comment       """The institution the currently owns the NVI result. Example UIO.
    We do not know whether the values of this field are standardized and whether there is a defined set of values for this property's range""" ;
    :currently_ignored "true" .


:status_kontrollert
    a                  :cristinfield ;
    rdfs:range         xsd:string ;
    rdfs:domain        :VITENSKAPELIGARBEID_LOKAL_Class ;
    rdfs:comment       """
     It refers to the respective institution's opinion on whether the Cristin entry should be reported to NVI and count towards RBK funding.
    NULL = this institution has not yet given their opinion
    J = this institution believes the current result should be included in the NVI report
    N = this institution believes the current result should NOT be included in the NVI report (e.g. doesn't meet academic standards, or has other issues)
    """ ;
    :currently_ignored "true" .

:brukernavn_kontrollert
    a                  :cristinfield ;
    rdfs:range         xsd:string ;
    rdfs:domain        :VITENSKAPELIGARBEID_LOKAL_Class ;
    rdfs:comment       """
     The username who controlled / judged / validated the respective entry representing  their respective institution,
     indicated  by the field VITENSKAPELIGARBEID_LOKAL.eierkode.
    """ ;
    :currently_ignored "true" .

:dato_kontrollert
    a                  :cristinfield ;
    rdfs:range         xsd:string ;
    rdfs:domain        :VITENSKAPELIGARBEID_LOKAL_Class ;
    rdfs:comment       """
     The date the respective entry was controlled by the user defined by the fields (brukernavn_kontrollert, eierkode) in the object VITENSKAPELIGARBEID_LOKAL.
    """ ;
    :currently_ignored "true" .

:status_bekreftet_arkivsporsmal
    a                  :cristinfield ;
    rdfs:range         xsd:string ;
    rdfs:domain        :VITENSKAPELIGARBEID_LOKAL_Class ;
    rdfs:comment       """UNKNOWN meaning""" ;
    :currently_ignored "true" .

:brukernavn_avlvrt_arkivsystem
    a                  :cristinfield ;
    rdfs:range         xsd:string ;
    rdfs:domain        :VITENSKAPELIGARBEID_LOKAL_Class ;
    rdfs:comment       """UNKNOWN meaning""" ;
    :currently_ignored "true" .

:dato_avlvrt_arkivsystem
    a                  :cristinfield ;
    rdfs:range         xsd:dateTimeStamp ;
    rdfs:domain        :VITENSKAPELIGARBEID_LOKAL_Class ;
    rdfs:comment       """UNKNOWN meaning""" ;
    :currently_ignored "true" .

:status_fulgt_medf_reg
    a                  :cristinfield ;
    rdfs:range         xsd:string ;
    rdfs:domain        :VITENSKAPELIGARBEID_LOKAL_Class ;
    rdfs:comment       """UNKNOWN meaning""" ;
    :currently_ignored "true" .

:brukernavn_svart_medforf_reg
    a                  :cristinfield ;
    rdfs:range         xsd:string ;
    rdfs:domain        :VITENSKAPELIGARBEID_LOKAL_Class ;
    rdfs:comment       """UNKNOWN meaning""" ;
    :currently_ignored "true" .

:dato_svart_medforf_regel
    a                  :cristinfield ;
    rdfs:range         xsd:string ;
    rdfs:domain        :VITENSKAPELIGARBEID_LOKAL_Class ;
    rdfs:comment       """UNKNOWN meaning""" ;
    :currently_ignored "true" .


:VARBEID_VDISIPLIN
    a            :cristinfield ;
    rdfs:comment "See description of domain class" ;
    rdfs:range   :VARBEID_VDISIPLIN_Class ;
    rdfs:domain  :Result .

:disiplinkode
    a            :cristinfield ;
    rdfs:comment """A code identifying a node in the VARBEID_VDISIPLIN tree.
        The specified node is the most fine grained description of the relevant discipline.
        The code is a number in the form of a string""" ;
    rdfs:range   xsd:string ;
    rdfs:domain  :VARBEID_VDISIPLIN_Class .

:disiplinkode_eier
    a            :cristinfield ;
    rdfs:comment "A code identifying the parent node of the respective publications discipline. The code is a number in the form of a string" ;
    rdfs:range   xsd:string ;
    rdfs:domain  :VARBEID_VDISIPLIN_Class .

:disiplinnavn_bokmal
    a            :cristinfield ;
    rdfs:comment "Name of the discipline in bokmal" ;
    rdfs:range   xsd:string ;
    rdfs:domain  :VARBEID_VDISIPLIN_Class .

:disiplinnavn_engelsk
    a            :cristinfield ;
    rdfs:comment "Name of the discipline in english" ;
    rdfs:range   xsd:string ;
    rdfs:domain  :VARBEID_VDISIPLIN_Class .

:disiplinnavn_nynorsk
    a            :cristinfield ;
    rdfs:comment "Name of the discipline in nynorsk" ;
    rdfs:range   xsd:string ;
    rdfs:domain  :VARBEID_VDISIPLIN_Class .

:TYPE_MEDIEBIDRAG
    a                  :cristinfield ;
    rdfs:range         :TYPE_MEDIEBIDRAG_Class ;
    rdfs:domain        :Result ;
    rdfs:comment       """A Cristin Result will have such a field only when its :varbeidunderkatkode has one of the following values:
	PROGLEDELSE, PROGDELTAGELSE, DOKUMENTAR, INTERVJU""" ;
    :currently_ignored true .

:varbeidlopenr
    a                  :cristinfield ;
    rdfs:range         xsd:integer ;
    rdfs:domain        :TYPE_MEDIEBIDRAG_Class ;
    rdfs:comment       """The Cristin Id of the respective :Result .

It is a self reference.""" ;
    :currently_ignored true .


:PRESENTASJON_VARBEID
    a                  :cristinfield ;
    rdfs:range         :PRESENTASJON_VARBEID_Class ;
    rdfs:domain        :Result ;
    rdfs:comment       """A project that the respective publication is part of.""" ;
    :currently_ignored false .

:presentasjonslopenr
    a                  :cristinfield ;
    rdfs:range         xsd:integer ;
    rdfs:domain        :PRESENTASJON_VARBEID_Class ;
    rdfs:comment       """ When the value of "presentasjonstypekode" is equal to :PRESENTASJONSTYPEKODE_PROSJEKT, it contains the project's Cristin ID.
    Otherwise its value has no meaning.
    """ ;
    :currently_ignored false .

:presentasjonstypekode
    a                  :cristinfield ;
    rdfs:range         :PRESENTASJONSTYPEKODE_VALUES_Class ;
    rdfs:domain        :PRESENTASJON_VARBEID_Class ;
    rdfs:comment       """
    When the value is equal to :PRESENTASJONSTYPEKODE_PROSJEKT, then it indicates that the respective PRESENTASJON_VARBEID_Class instance
    is a reference to a Cristin project.
    When the value is equal to :PRESENTASJONSTYPEKODE_PERSON, it indicates that it belongs to the collection of "important", "preferred"
    publications of the author.
    """ ;
    :currently_ignored false .

:finansieringslopenr
    a                  :cristinfield ;
    rdfs:range         xsd:integer ;
    rdfs:domain        :FINANSIERING_VARBEID_Class ;
    rdfs:comment       """Internal Cristin ID of a funding entry / research grant.
    Can be dereferenced at https://api.cristin.no/v2/fundings/<finansieringslopenr>
    """ ;
    :currently_ignored true .

:finansieringskildekode
    a                  :cristinfield ;
    rdfs:range         xsd:string ;
    rdfs:domain        :FINANSIERING_VARBEID_Class ;
    rdfs:comment       """Code representing the funding body that awarded the research grant.
    Possible values include "EU","NFR".
    A list of possible values can be found at https://api.cristin.no/v2/fundings/sources?lang=en,nb,nn
    """ ;
    :currently_ignored true .

:finansieringsreferanse
    a                  :cristinfield ;
    rdfs:range         xsd:integer ;
    rdfs:domain        :FINANSIERING_VARBEID_Class ;
    rdfs:comment       """The external entry id of the research grant, used by the funding body.""" ;
    :currently_ignored true .

:belop
    a                  :cristinfield ;
    rdfs:range         rdf:nil ; # Always empty
    rdfs:domain        :FINANSIERING_VARBEID_Class ;
    rdfs:comment       """The amount of money awarded in this grant. This field is always empty.""" ;
    :currently_ignored true .

:arstall_fra
    a                  :cristinfield ;
    rdfs:range         xsd:integer ;
    rdfs:domain        :FINANSIERING_VARBEID_Class ;
    rdfs:comment       """Year the funding / research grant started""" ;
    :currently_ignored true .

:arstall_til
    a                  :cristinfield ;
    rdfs:range         xsd:integer ;
    rdfs:domain        :FINANSIERING_VARBEID_Class ;
    rdfs:comment       """Year the funding / research grant ended.""" ;
    :currently_ignored true .



:type_bok_rapport
    a               :cristinfield ;
    rdfs:range      :TYPE_BOK_RAPPORT_Class ;
    rdfs:domain     :Result ; .



:isbn
    a               :cristinfield ;
    rdfs:comment    "The isbn which the respective book is registered with. Is nullable when the domain is :TIDSSKRIFTSERIE_Class." ;
    rdfs:range      xsd:string ;
    rdfs:domain     :TYPE_BOK_RAPPORT_Class ; .

:utgivernavn
    a               :cristinfield ;
    rdfs:comment    "The name of the publisher of the respective book. Can be empty." ;
    rdfs:range      xsd:string ;
    rdfs:domain     :TYPE_BOK_RAPPORT_Class ; .

:forlag
    a            :cristinfield ;
    rdfs:comment """
        Information about the Publishing House of the respective Book or Report.
        The connection between the subfields forlag.forlagsnavn and utgivernavn is UNKNONWN.
         There are 353 cases where forlag.forlagsnavn and utgivernavn are not the same and there is no NSD code for reference.
         There are also about 140 000 cases where there is no forlag entry but there is utgivernavn.

        """ ;
    rdfs:range   :FORLAG_Class ;
    rdfs:domain  :TYPE_BOK_RAPPORT_Class .

:forlagsnavn
    a            :cristinfield ;
    rdfs:range   xsd:string ;
    rdfs:domain  :FORLAG_Class ;
    rdfs:comment """The name of the Publishing House that published the book""" .

:forlagsnr
    a            :cristinfield ;
    rdfs:range   xsd:integer ;
    rdfs:domain  :FORLAG_Class ;
    rdfs:comment """The internal Cristin number of the specific Book  series.""" ;
    :should_ignore   true.


:fagfelt
    a            :cristinfield ;
    rdfs:comment "The scientific field in which the book is published" ;
    rdfs:range   :FAGFELT_Class ;
    rdfs:domain  :TYPE_BOK_RAPPORT_Class .


:tidsskrift_serie
    a            :cristinfield ;
    rdfs:comment """
        A Publisher's series that is modeled by NSD as Journal. Probably not exactly a journal since the respective Cristin Results are Books or Reports.
        This field has the exact same structure as the field "tidskrift" in the field "type_tidsskriftpublikasjon"
     """ ;
    rdfs:range   :TIDSSKRIFT_Class ;
    rdfs:domain  :TYPE_BOK_RAPPORT_Class .

:fagfeltkode
    a               :cristinfield ;
    rdfs:comment    "The (numerical) code representing the scientific field in which the book is published" ;
    rdfs:range      xsd:positiveInteger ;
    rdfs:domain     :FAGFELT_Class ; .

:fagomradekode
    a                  :cristinfield ;
    rdfs:comment       "The (abbreviation) code representing the scientific field in which the book is published" ;
    rdfs:range         xsd:string ;
    rdfs:domain        :FAGFELT_Class ;
    :currently_ignored "true" .

:navn
    a                  :cristinfield ;
    rdfs:comment       "The NSD name of the scientific field in which the book is published" ;
    rdfs:range         xsd:string ;
    rdfs:domain        :FAGFELT_Class ;
    :currently_ignored "true" .

:navn_engelsk
    a                  :cristinfield ;
    rdfs:comment       "The english name of the scientific field in which the book is published" ;
    rdfs:range         xsd:string ;
    rdfs:domain        :FAGFELT_Class ;
    :currently_ignored "true" .

:type_tidsskriftpublikasjon
    a               :cristinfield ;
    rdfs:comment    """
    A type publication called tidsskrift.
    """ ;
    rdfs:range      :TYPE_TIDSSKRIFTPUBLIKASJON_Class ;
    rdfs:domain     :Result ; .

:volum
    a               :cristinfield ;
    rdfs:comment    """
    The volume in which the article is published. The value is a number in the form of a string. Possibly null.
    """ ;
    rdfs:range      xsd:string ;
    rdfs:domain     :TYPE_TIDSSKRIFTPUBLIKASJON_Class ; .

:sidenr_fra
    a               :cristinfield ;
    rdfs:comment    "The page number the that marks the start of the article. The value is a number in the form of a string. Possibly null." ;
    rdfs:range      xsd:string ;
    rdfs:domain     :TYPE_TIDSSKRIFTPUBLIKASJON_Class ; .

:sidenr_til
    a               :cristinfield ;
    rdfs:comment    "The page number the that marks the end of the article. The value is a number in the form of a string. Possibly null." ;
    rdfs:range      xsd:string ;
    rdfs:domain     :TYPE_TIDSSKRIFTPUBLIKASJON_Class ; .

:doi
    a               :cristinfield ;
    rdfs:comment    "The doi connected to the respective entry. Possibly null." ;
    rdfs:range      xsd:string ;
    rdfs:domain     :TYPE_TIDSSKRIFTPUBLIKASJON_Class, :TYPE_BOK_RAPPORT_DEL_Class ; .

:antall_sider_totalt
    a               :cristinfield ;
    rdfs:comment    """
    The total number of pages of the specific entry.
    When the the entry represents a part of another entry (e.g. a Chapter in a Book) then the total number of pages
    refers to the entry (e.g Chapter) and not the to parent entry (e.g. Book).
    """ ;
    rdfs:range      xsd:positiveInteger ;
    rdfs:domain     :TYPE_BOK_RAPPORT_Class, :TYPE_TIDSSKRIFTPUBLIKASJON_Class, :TYPE_BOK_RAPPORT_DEL_Class ; .

:publiseringsar
    a                  :cristinfield ;
    rdfs:comment       """
    The year of publication for the Cristin Result. In 99% of the results it is the same as the "arstall".
    It can be safely ignored.
     """ ;
    rdfs:range         xsd:positiveInteger ;
    rdfs:domain        :TYPE_TIDSSKRIFTPUBLIKASJON_Class ;
    :currently_ignored "true" ;
    :should_ignore     "true" .


:hefte
    a                  :cristinfield ;
    rdfs:comment       """
        The issue containing the publication.
        A string holding information about the which issue it is,
        this could be in the form of a number, a roman number or any other way of distinguishing an issue""" ;
    rdfs:range         xsd:string ;
    rdfs:domain        :TYPE_TIDSSKRIFTPUBLIKASJON_Class ;
    :currently_ignored "true" .

:status_referee_ordning
    a                  :cristinfield ;
    rdfs:comment       "Defines whether or not the Journal is peerreviewed (J)=yes, (N)=no and NULL." ;
    rdfs:range         xsd:string ;
    rdfs:domain        :TYPE_TIDSSKRIFTPUBLIKASJON_Class ;
    :currently_ignored "true" .

:supplement
    a                  :cristinfield ;
    rdfs:comment       "A area for adding information about possible attachments to the article." ;
    rdfs:range         xsd:string ;
    rdfs:domain        :TYPE_TIDSSKRIFTPUBLIKASJON_Class ;
    :currently_ignored "true" .

:utbredelsesomrade
    a                  :cristinfield ;
    rdfs:comment       """
        Information about where or to what extent the article has been published.
        Examples: NORSK, NORDISK, INTERNASJ, NASJONALT, UKJENT""" ;
    rdfs:range         xsd:string ;
    rdfs:domain        :TYPE_TIDSSKRIFTPUBLIKASJON_Class ;
    :currently_ignored "true" .

:artikkelnummer
    a                  :cristinfield ;
    rdfs:comment       """
        A string identifying the article within the journal.
        Possibly null.
        """ ;
    rdfs:range         xsd:string ;
    rdfs:domain        :TYPE_TIDSSKRIFTPUBLIKASJON_Class ;
    :currently_ignored "true" .

:arstall_trykket
    a                  :cristinfield ;
    rdfs:comment       "The year the publication was printed." ;
    rdfs:range         xsd:positiveInteger ;
    rdfs:domain        :TYPE_TIDSSKRIFTPUBLIKASJON_Class ;
    :currently_ignored "true" .

:arstall_online
    a                  :cristinfield ;
    rdfs:comment       "The year the publication was released online." ;
    rdfs:range         xsd:positiveInteger ;
    rdfs:domain        :TYPE_TIDSSKRIFTPUBLIKASJON_Class ;
    :currently_ignored "true" .

:tidskrift
    a            :cristinfield ;
    rdfs:comment """See description in range class.""" ;
    rdfs:range   :TIDSSKRIFT_Class ;
    rdfs:domain  :TYPE_TIDSSKRIFTPUBLIKASJON_Class .

:issn
    a               :cristinfield ;
    rdfs:comment    "The issn connected to the respective article. Possibly null." ;
    rdfs:range      xsd:string ;
    rdfs:domain     :TIDSSKRIFT_Class ; .

:issn_elektronisk
    a               :cristinfield ;
    rdfs:comment    "The online version of the issn connected to the respective article. Possibly null." ;
    rdfs:range      xsd:string ;
    rdfs:domain     :TIDSSKRIFT_Class ; .

:tidsskriftnavn
    a               :cristinfield ;
    rdfs:comment    "The name of the journal publishing the article" ;
    rdfs:range      xsd:string ;
    rdfs:domain     :TIDSSKRIFT_Class ; .

:tidsskriftnr
    a                  :cristinfield ;
    rdfs:comment       "Number identifying the specific journal within Cristin" ;
    rdfs:range         xsd:positiveInteger ;
    rdfs:domain        :TIDSSKRIFT_Class ;
    :currently_ignored "true" .

:nsdkode

    a            :cristinfield ;
    rdfs:comment "A code representing the id of a Journal, Series (also viewed as a Journal in NSD) or Publishing House in NSD-channel registry " ;
    rdfs:range   rdf:nil ; #unknown range
    rdfs:domain  :TIDSSKRIFT_Class, :FORLAG_Class  ;
    :currently_ignored   "false" .

:landkode_utgiver
    a                  :cristinfield ;
    rdfs:comment       """
        The code identifying the country where the publisher is located.
        Example: NO
        Possibly null.""" ;
    rdfs:range         xsd:string ;
    rdfs:domain        :TIDSSKRIFT_Class ;
    :currently_ignored "true" .

:status_referee_ordning
    a                  :cristinfield ;
    rdfs:comment       "Defines whether or not the Journal is peerreviewed (J)=yes, (N)=no, (U)=uncertain and NULL." ;
    rdfs:range         xsd:string ;
    rdfs:domain        :TIDSSKRIFT_Class ;
    :currently_ignored "true" .

:dato_utgatt
    a                  :cristinfield ;
    rdfs:comment       """If the journal no longer exists this is the date when it disapeared.
    Information about what if any: replaced it, it merged into, or what it developed into.
    Info can be found with NSD and Cristin but is not exported as of today.
    """ ;
    rdfs:range         xsd:string ;
    rdfs:domain        :TIDSSKRIFT_Class ;
    :currently_ignored "true" .

:status_serie
    a                  :cristinfield ;
    rdfs:comment       """When the value is N, this TIDSSKRIFT object represents a journal.
    When the value is J, this TIDSSKRIFT object represents a book series.
    Objects with value J are not expected to be referred to from a TYPE_TIDSSKRIFTPUBLIKASJON object.
    Objects with value J are only expected to be referred to from a TYPE_BOK_RAPPORT object.
    """ ;
    rdfs:range         xsd:string ;
    rdfs:domain        :TIDSSKRIFT_Class ;
    :currently_ignored "true" .

:VARBEID_EMNEORD
    a               :cristinfield ;
    rdfs:comment    """See the range class.""" ;
    rdfs:range      :VARBEID_EMNEORD_Class ;
    rdfs:domain     :Result ; .

:emneordnavn_bokmal
    a               :cristinfield ;
    rdfs:comment    """
    The bokmal version of the VARBEID_EMNEORD. Possibly null.
    """ ;
    rdfs:range      xsd:string ;
    rdfs:domain     :VARBEID_EMNEORD_Class ; .

:emneordnavn_engelsk
    a               :cristinfield ;
    rdfs:comment    "The english version of the VARBEID_EMNEORD. Possibly null." ;
    rdfs:range      xsd:string ;
    rdfs:domain     :VARBEID_EMNEORD_Class ; .

:emneordnavn_nynorsk
    a               :cristinfield ;
    rdfs:comment    "The nynorsk version of the the VARBEID_EMNEORD. Possibly null." ;
    rdfs:range      xsd:string ;
    rdfs:domain     :VARBEID_EMNEORD_Class ; .

:helsekategorikode
    a                  :cristinfield ;
    rdfs:comment       """Health Category Code in the UKCRC Health Research Classification System (HRCS).
    See https://hrcsonline.net/health-categories/.
    """ ;
    rdfs:range         xsd:string ;
    rdfs:domain        :VARBEID_HRCS_KLASSIFISERING_Class ; .

:aktivitetskode
    a                  :cristinfield ;
    rdfs:comment       """Research Activity Code in the UKCRC Health Research Classification System (HRCS).
                     See https://hrcsonline.net/research-activities/.
                     """ ;
    rdfs:range         xsd:string ;
    rdfs:domain        :VARBEID_HRCS_KLASSIFISERING_Class ; .

:TYPE_BOK_RAPPORT_DEL
    a            :cristinfield ;
    rdfs:comment """Reference to a Cristin entry that is a part of a book or report.""" ;
    rdfs:range   :TYPE_BOK_RAPPORT_Class ;
    rdfs:domain  :Result .

:varbeidlopenr_inngar_i
    a            :cristinfield ;
    rdfs:comment """The CristinID of the current TYPE_BOK_RAPPORT_DEL_Class entry's parent TYPE_BOK_RAPPORT_Class entry.""" ;
    rdfs:domain  :TYPE_BOK_RAPPORT_DEL_Class ;
    rdfs:range   xsd:integer .

:status_utgitt_av_forlag
    a            :cristinfield ;
    rdfs:comment """UNKNOWN meaning. It takes values "J" and "N" corresponding to the values true and false.""" ;
    rdfs:range   xsd:string ;
    rdfs:domain  :TYPE_BOK_RAPPORT_DEL_Class .

:delangivelse
    a                  :cristinfield ;
    rdfs:comment       """A free text comment describing the relation of the respective Result to the parent entry.
    Example values: Session 2   Chapter 2, Introduction, Del I: Kunsten som metodisk univers/Kapittel 3
    Suggestion: to be ignored.
    """ ;
    rdfs:range         xsd:string ;
    rdfs:domain        :TYPE_BOK_RAPPORT_DEL_Class ;
    :currently_ignored true .

:sidenr_fra
    a            :cristinfield ;
    rdfs:comment """The starting page of the part in the respective parent entry.
    Expressed as a string to cover roman numerals or other non-integer ways of denoting pages.
    """ ;
    rdfs:range   xsd:string ;
    rdfs:domain  :TYPE_BOK_RAPPORT_DEL_Class .

:sidenr_til
    a            :cristinfield ;
    rdfs:comment """The ending page of the part in the respective parent entry.
    Expressed as a string to cover roman numerals or other non-integer ways of denoting pages.
    """ ;
    rdfs:range   xsd:string ;
    rdfs:domain  :TYPE_BOK_RAPPORT_DEL_Class .

:sprakkode_oversatt_fra
    a            :cristinfield ;
    rdfs:comment """It has meaning only when the respective entry has :varbeidunderkatkode OVERSETTELSE_KAP
    or OVERSETTELSE_BOK, indicating that the current entry is a translation of a book or chapter.
 The value represents the language of the original document as an ISO 639-1 code. The original document is not
 referenced further as it may not be in the scope of Cristin.
  """ ;
    rdfs:range   xsd:string ;
    rdfs:domain  :TYPE_BOK_RAPPORT_Class, :TYPE_BOK_RAPPORT_DEL_Class .
