@prefix rdf:    <http://www.w3.org/1999/02/22-rdf-syntax-ns#> .
@prefix rdfs:   <http://www.w3.org/2000/01/rdf-schema#> .
@prefix xsd:    <http://www.w3.org/2001/XMLSchema#> .
@prefix :       <http://www.example.com/cristin-ontology#> .

#Info about rdfs types
#https://www.w3.org/TR/rdf-schema/#ch_resource


:NvaClass
    a            rdfs:Class ;
    rdfs:comment "Any class that represents an entity or collection of values in NVA" .

:CristinClass
    a            rdfs:Class ;
    rdfs:comment "Any class that represent an entity or collection of values in Cristin" .

:Result
    a               :CristinClass ;
    rdfs:subClassOf :CristinClass ;
    rdfs:comment    "The equivalent of an NVA Resource in Cristin. An entry as being exported especially for importing in NVA" .

:PublicationStatus
    a :CristinClass .

:Published
    a               :CristinClass ;
    rdfs:label      "PUBLISHED" ;
    rdfs:subClassOf :PublicationStatus ;
    rdfs:subClassOf :CristinClass .


:VARBEID_SPRAK_Class
    a               :CristinClass ;
    rdfs:comment    "The structure defining the VARBEID_SPRAK property." ;
    rdfs:subClassOf :CristinClass .

:VARBEID_PERSON_Class
    a               :CristinClass ;
    rdfs:comment    """
    The structure of the VARARBEID_PERSON entry. It contains information about the status of the contributor
    at the time the Result was registered in Cristin.
    """ ;
    rdfs:subClassOf :CristinClass .


:VARBEID_PERSON_STED_Class
    a               :CristinClass ;
    rdfs:comment    """
    The structure of the VARBEID_PERSON_STED entry.
    It contains information about the status of a contributor's institution at the time the Result
    was registered in Cristin. It is uncertain whether the contributor presently belongs to the same institution,
    or if the institution status has changed.
    """ ;
    rdfs:subClassOf :CristinClass .

:VARBEID_PERSON_STED_ROLLE_Class
    a               :CristinClass ;
    rdfs:comment    """
     The structure of VARBEID_PERSON_STED_ROLLE. It contains information about the role of
    the contributor in their institution at the time the Result was registered in Cristin. It is uncertain
    whether the contributor presnetly holds the same role, or they belong to the same institution, or the
    role still exists, or the institution's status has changed.
    """ ;
    rdfs:subClassOf :CristinClass .



:cristinField
    a            rdf:Property ;
    rdfs:comment "Any property of any Cristin class" ;
    rdfs:domain  :CristinClass ;
    rdfs:range   rdfs:Class .


:nvaField
    a            rdf:Property ;
    rdfs:comment "Any property of any NVA class" ;
    rdfs:domain  :NvaClass ;
    rdfs:range   rdfs:Class .


:mapsToNvaField
    a           rdf:Property ;
    rdfs:range  xsd:string ;
    rdfs:domain :cristinField .

:isIgnored
    a           rdf:Property ;
    rdfs:range  xsd:boolean ;
    rdfs:domain :cristinField .



:id
    a               :cristinField ;
    rdfs:comment    "Identifier of Cristin Result entry." ;
    rdfs:range      xsd:positiveInteger ;
    rdfs:domain     :Result ;
    :mapsToNvaField """
        "additionalIdentifiers":[
            {
                "source":"Cristin",
                "value": ":id"
            }
        ]
    """ .

:arstall
    a               :cristinField ;
    rdfs:comment    "The year a resource (result) was published." ;
    rdfs:range      xsd:positiveInteger ;
    rdfs:domain     :Result ;
    :mapsToNvaField """
        entityDescription.date.year = :arstall;
        entityDescription.date.month = null;
        entityDescription.date.day = null;
    """ .

:dato_opprettet
    a               :cristinField ;
    rdfs:comment    "The date the resource was registered in Cristin." ;
    rdfs:range      xsd:date ;
    rdfs:domain     :Result ;
    :mapsToNvaField "createdDate" .

:varbeidhovedkatkode
    a               :cristinField ;
    rdfs:comment    """
    The main category of the resource,
    The range of this property is found here: https://api.cristin.no/v2/results/categories?lang=nb,en
    """ ;
    rdfs:range      xsd:string ;
    rdfs:domain     :Result ;
    :mapsToNvaField "practically not in use because :varbeidunderkatkode can specify the type of publication" .

:varbeidunderkatkode
    a               :cristinField ;
    rdfs:comment    "The secondary category of the resource. No specific range available at the moment." ;
    rdfs:range      xsd:string ;
    rdfs:domain     :Result ;
    :mapsToNvaField """
    entityDescription.reference.publicationInstance
        Anthology -> BookAnthology
    """ .

:eierkode_opprettet
    a            :cristinField ;
    rdfs:comment "The institution of the person who created the first version of the registration." ;
    rdfs:range   xsd:string ;
    rdfs:domain  :Result ;
    :isIgnored   "true" .


:eierkode_siste_endring
    a            :cristinField ;
    rdfs:comment "The institution of the person who edited last the registration." ;
    rdfs:range   xsd:string ;
    rdfs:domain  :Result ;
    :isIgnored   "true" .

:dato_siste_endring
    a            :cristinField ;
    rdfs:comment "The date of the last update of the registration." ;
    rdfs:range   xsd:date ;
    rdfs:domain  :Result ;
    :isIgnored   "true" .



:publiseringstatuskode
    a               :cristinField ;
    rdfs:comment    """
    The publication status of the entry in Cristin, i.e., whether the metadata are publicly available or not.
    This status is not related to the status of the actual data, e.g. whether the actual material has been
    published by some publisher (e.g. Elsevier).
    """ ;
    rdfs:range      :Published ; # it can only be "PUBLISERT"
    rdfs:domain     :Result ;
    :mapsToNvaField "status = PUBLISHED " .


:dato_utgitt
    a            :cristinField ;
    rdfs:comment "Date the resource was published (e.g. through Elsevier or in OpenAccess Journal)." ;
    rdfs:range   xsd:date ;
    rdfs:domain  :Result ;
    :isIgnored   "true" .

:arstall_rapportert
    a            :cristinField ;
    rdfs:comment "Year that the resource was registered in Cristin." ;
    rdfs:range   xsd:positiveInteger ;
    rdfs:domain  :Result ;
    :isIgnored   "true" .



:merknadtekst
    a            :cristinField ;
    rdfs:comment "UNKNOWN property." ;
    rdfs:range   xsd:string ;
    rdfs:domain  :Result ;
    :isIgnored   "true" .

:merknadtekst_godkjenning
    a            :cristinField ;
    rdfs:comment "UNKNOWN property." ;
    rdfs:range   xsd:string ;
    rdfs:domain  :Result ;
    :isIgnored   "true" .

:kildekode
    a            :cristinField ;
    rdfs:comment "UNKNOWN property." ;
    rdfs:range   xsd:anyURI ;
    rdfs:domain  :Result .

:kildepostid
    a            :cristinField ;
    rdfs:comment "UNKNOWN property." ;
    rdfs:range   xsd:anyURI ;
    rdfs:domain  :Result ;
    :isIgnored   "true" .

:pubidnr
    a            :cristinField ;
    rdfs:comment "UNKNOWN property." ;
    rdfs:range   xsd:positiveInteger ;
    rdfs:domain  :Result ;
    :isIgnored   "true" .

:VARBEID_SPRAK
    a               :cristinField ;
    rdfs:comment    """
    A language that this work has been published in, the respective title, and the respective abstract
    and an indication whether it is the original language or a translation.
    """ ;
    rdfs:range      :VARBEID_SPRAK_Class ;
    rdfs:domain     :Result ;
    :mapsToNvaField """
        entityDescription.mainTitle, entityDescription.language
    """ .

:sprakkode
    a               :cristinField ;
    rdfs:comment    """
    The language of the title and the abstract included in the VARARBEID_SPRAK entry.
    The range could possibly be an xsd:language.
    """ ;
    rdfs:range      xsd:string ;
    rdfs:domain     :VARBEID_SPRAK_Class ;
    :mapsToNvaField """
        entityDescription.language if VARBEID_SPRAK.status_original is "J"
    """ .

:tittletekst
    a               :cristinField ;
    rdfs:comment    "The title in the VARARBEID_SPRAK entry. It is supposed to be in the language described by :sprakkode" ;
    rdfs:range      xsd:string ;
    rdfs:domain     :VARBEID_SPRAK_Class ;
    :mapsToNvaField """
        entityDescription.mainTitle  if VARBEID_SPRAK.status_original is "J"
    """ .


:sammendragtekst
    a            :cristinField ;
    rdfs:comment "The abstract in the VARARBEID_SPRAK entry. It is supposed to be in the language described by :sprakkode" ;
    rdfs:range   xsd:string ;
    rdfs:domain  :VARBEID_SPRAK_Class ;
    :isIgnored   "true" .

:status_original
    a            :cristinField ;
    rdfs:comment """
    Indicator of whether the title in the respective VARBEID_SPRAK is the original title or not.
    Known possible values are 'J' (which is possibly a representation for the boolean value 'true').
    """ ;
    rdfs:range   xsd:string ;
    rdfs:domain  :VARBEID_SPRAK_Class ;
    :isIgnored   "false" .

:VITENSKAPELIGARBEID_LOKAL
    a            :cristinField ;
    rdfs:comment "UNKONWN property" ;
    rdfs:domain  :Result ;
    :isIgnored   "true" .

:VARBEID_PERSON
    a               :cristinField ;
    rdfs:comment    "A contributor to the respective result entry." ;
    rdfs:range      :VARBEID_PERSON_Class ;
    rdfs:domain     :Result ;
    :mapsToNvaField "entityDescription.Contributor" .

:personlopenr
    a               :cristinField ;
    rdfs:comment    "The Cristin Person identifier of the contributor" ;
    rdfs:range      xsd:positiveInteger ;
    rdfs:domain     :VARBEID_PERSON_Class ;
    :mapsToNvaField "entityDescription.contributor.identity.id" .

:fornavn
    a               :cristinField ;
    rdfs:comment    "The first/given name of the contributor of the respective result entry" ;
    rdfs:range      xsd:string ;
    rdfs:domain     :VARBEID_PERSON_Class ;
    :mapsToNvaField "entityDescription.contributor.identity.fullanme" .

:etternavn
    a               :cristinField ;
    rdfs:comment    "The surname/family-name of the contributor of the respective result entry" ;
    rdfs:range      xsd:string ;
    rdfs:domain     :VARBEID_PERSON_Class ;
    :mapsToNvaField "entityDescription.contributor.fullanme" .

:VARBEID_PERSON_STED
    a               :cristinField ;
    rdfs:comment    """
    Details about the institution which the contributor belongs to and the contributors role to the institution
    at the time the publication was registered in Cristin.
    """ ;
    rdfs:range      :VARBEID_PERSON_STED_Class ;
    rdfs:domain     :VARBEID_PERSON_Class ;
    :mapsToNvaField "entityDescription.contributor.affiliation" .


:institusjonsnr
    a               :cristinField ;
    rdfs:comment    "The Cristin institution identifier of the respective institution." ;
    rdfs:range      xsd:positiveInteger ;
    rdfs:domain     :VARBEID_PERSON_STED_Class ;
    :mapsToNvaField "entityDescription.contributor.affiliation.id" .

:avdnr
    a               :cristinField ;
    rdfs:comment    "Department number. More information about the origin of the number is necessary" ;
    rdfs:range      xsd:positiveInteger ;
    rdfs:domain     :VARBEID_PERSON_STED_Class ;
    :mapsToNvaField "entityDescription.contributor.affiliation.id" .

:undavdnr
    a               :cristinField ;
    rdfs:comment    "Sub-department number. More information about the origin of the number is necessary." ;
    rdfs:range      xsd:positiveInteger ;
    rdfs:domain     :VARBEID_PERSON_STED_Class ;
    :mapsToNvaField "entityDescription.contributor.affiliation.id" .

:gruppenr
    a               :cristinField ;
    rdfs:comment    "UNKNOWN property" ;
    rdfs:range      xsd:positiveInteger ;
    rdfs:domain     :VARBEID_PERSON_STED_Class ;
    :mapsToNvaField "entityDescription.contributor.affiliation.id" .

:stedkode_opprinnelig
    a            :cristinField ;
    rdfs:comment "UNKNOWN property" ;
    rdfs:range   xsd:positiveInteger ;
    rdfs:domain  :VARBEID_PERSON_STED_Class ;
    :isIgnored   "true" .

:institusjonsnavn_opprinnelig
    a            :cristinField ;
    rdfs:comment "UNKNOWN property" ;
    rdfs:range   xsd:positiveInteger ;
    rdfs:domain  :VARBEID_PERSON_STED_Class ;
    :isIgnored   "true" .

:avdelingsnavn_opprinnelig
    a            :cristinField ;
    rdfs:comment "UNKNOWN property" ;
    rdfs:range   xsd:string ;
    rdfs:domain  :VARBEID_PERSON_STED_Class ;
    :isIgnored   "true" .

:stednavn_opprinnelig
    a            :cristinField ;
    rdfs:comment "UNKNOWN property" ;
    rdfs:range   xsd:string ;
    rdfs:domain  :VARBEID_PERSON_STED_Class ;
    :isIgnored   "true" .

:vekting
    a            :cristinField ;
    rdfs:comment "UNKNOWN property" ;
    rdfs:range   rdf:nil ; #unknown range
    rdfs:domain  :VARBEID_PERSON_STED_Class ;
    :isIgnored   "true" .

:VARBEID_PERSON_STED_ROLLE
    a               :cristinField ;
    rdfs:comment    """
        The role of the respective person in the respective institution at the time the respective Result was registered in
        Cristin.
        """ ;
    rdfs:range      :VARBEID_PERSON_STED_ROLLE_Class ;
    rdfs:domain     :VARBEID_PERSON_STED_Class ;
    :mapsToNvaField "entityDescription.contributor.role" .

:rollekode
    a            :cristinField ;
    rdfs:comment "The role-code of the role of the contributor at the respective institution for the specific Result." ;
    rdfs:range   xsd:string ;
    rdfs:domain  :VARBEID_PERSON_STED_ROLLE_Class ;
    :isIgnored   "false" .


