@prefix rdf:    <http://www.w3.org/1999/02/22-rdf-syntax-ns#> .
@prefix rdfs:   <http://www.w3.org/2000/01/rdf-schema#> .
@prefix xsd:    <http://www.w3.org/2001/XMLSchema#> .
@prefix :       <http://www.example.com/cristin-ontology#> .

#Info about rdfs types
#https://www.w3.org/TR/rdf-schema/#ch_resource

:CristinClass
    a            rdfs:Class ;
    rdfs:label   "CristinClass" ;
    rdfs:comment "Any class that represent an entity or collection of values in Cristin" .

:Result
    a               :CristinClass ;
    rdfs:subClassOf :CristinClass ;
    rdfs:comment    "The equivalent of an NVA Resource in Cristin. An entry as being exported especially for importing in NVA" .

:PublicationStatus
    a :CristinClass .

:Published
    a               rdfs:Class ;
    rdfs:label      "PUBLISERT" ;
    rdfs:subClassOf :PublicationStatus .

:InPress
    a               rdfs:Class ;
    rdfs:label      "IN_PRESS" ;
    rdfs:subClassOf :PublicationStatus .

:TestPublicationStatus
    a               rdfs:Class ;
    rdfs:label      "TEST" ;
    rdfs:subClassOf :PublicationStatus .


:VARBEID_SPRAK_Class
    a               rdfs:Class ;
    rdfs:subClassOf :CristinClass ;
    rdfs:comment    "The structure defining the VARBEID_SPRAK property." .

:VARBEID_PERSON_Class
    a            rdfs:Class ;
    rdfs:comment """
    The structure of the VARARBEID_PERSON entry. It contains user submitted information about the status of the contributor
    at the time the Result was registered in Cristin. Some of the information can be  provided by the user manually in order to reflect the
    user's name at the time the manuscript/publication was submitted to the publisher (e.g. Elsevier).
    """ .


:VARBEID_PERSON_STED_Class
    a               rdfs:Class ;
    rdfs:subClassOf :CristinClass ;
    rdfs:comment    """
    The structure of the VARBEID_PERSON_STED entry.
    The entry contains information about the contributor's institutional affiliation represented in the result entity
     at the time of publication, as well as the current instance of that institution, should it have evolved over time.
    """ .


:VARBEID_PERSON_STED_ROLLE_Class
    a               rdfs:Class ;
    rdfs:subClassOf :CristinClass ;
    rdfs:comment    """
     The structure of VARBEID_PERSON_STED_ROLLE. It contains information about the role of
    the contributor in this publication. One contributor can have many different contribution roles from the same or different institutions.
    Example:
    Contributor C has contributed as "EDITOR" affiliated with InstA for publication P
    and they have contributed as "ILLUSTRATOR" affiliated with InstB for the same publication.
    """ .


:TYPE_MEDIEBIDRAG_Class
    a               rdfs:Class ;
    rdfs:subClassOf :CristinClass ;
    rdfs:comment    """
    The structure of TYPE_MEDIEBIDRAG.
            """ .

:PRESENTASJON_VARBEID_Class
    a               rdfs:Class ;
    rdfs:subClassOf :CristinClass ;
    rdfs:comment    """
    Reference to a project when :presentasjonstypekode is equal to :PRESENTASJONSTYPEKODE_PROSJEKT. More information in the
    description of the field :presentasjonstypekode.
    """ .

:PRESENTASJONSTYPEKODE_VALUES_Class
    a rdfs:Class .


:PRESENTASJONSTYPEKODE_PERSON
    a               rdfs:Class ;
    rdfs:label      "PERSON" ;
    rdfs:comment    "Indicates reference to a Cristin person Id. " ;
    rdfs:subClassOf :PRESENTASJONSTYPEKODE_VALUES_Class .

:PRESENTASJONSTYPEKODE_GRUPPE
    a               rdfs:Class ;
    rdfs:label      "GRUPPE" ;
    rdfs:comment    "UNKNOWN MEANING. When :presentasjonstypekode has this value, the reference is not a project." ;
    rdfs:subClassOf :PRESENTASJONSTYPEKODE_VALUES_Class .


:PRESENTASJONSTYPEKODE_PROSJEKT
    a               rdfs:Class ;
    rdfs:label      "PROSJEKT" ;
    rdfs:comment    "Indicates that the respective PRESENTASJON_VARBEID_Class instance is a reference to a Cristin project" ;
    rdfs:domain     :Result ;
    rdfs:subClassOf :PRESENTASJONSTYPEKODE_VALUES_Class .

:PRESENTASJONSTYPEKODE_ENHET
    a               rdfs:Class ;
    rdfs:label      "ENHET" ;
    rdfs:comment    "UNKNOWN MEANING. When :presentasjonstypekode has this value, the reference is not a project." ;
    rdfs:subClassOf :PRESENTASJONSTYPEKODE_VALUES_Class .

:PRESENTASJONSTYPEKODE_SENTER
    a               rdfs:Class ;
    rdfs:label      "SENTER" ;
    rdfs:comment    "UNKNOWN MEANING. When :presentasjonstypekode has this value, the reference is not a project." ;
    rdfs:subClassOf :PRESENTASJONSTYPEKODE_VALUES_Class .

:VARBEID_KILDE_Class
    a               rdfs:Class ;
    rdfs:subClassOf :CristinClass ;
    rdfs:comment    """
         When this entry is populated, the respective entry is imported from another source.
         E.g. FORSKDOK or SCOPUS a predecessor of Cristin
         """ .

:VITENSKAPELIGARBEID_LOKAL_Class
    a               rdfs:Class ;
    rdfs:subClassOf :CristinClass ;
    rdfs:comment    """
        This field contains metadata relevant for NVI reporting, one set per contributing institution that is also part of the NVI process.
        The contained metadata are related to the users that created/updated the entry for the NVI report. For example "brukernavn_opprettet"
        refers to the superuser that created the NVI entry and not the user that created the Cristin entry.
    """ .

:TYPE_BOK_RAPPORT_Class
    a               rdfs:Class ;
    rdfs:subClassOf :CristinClass ;
    rdfs:comment    """
         The respetive object contains metadata about a book.
         The respective field (TYPE_BOK_RAPPORT) has a value only if the varbeidhovedkatkode has one of the following values:
         OVERSETTELSESARB
         RAPPORT
         BOK.
         The Cristin secondary categories (varbeidunderkatkode)
         that are expected to have such an entry are the following:
         ANTOLOGI
         DRGRADAVH
         FAGBOK
         FORSKERLINJEOPPG
         HOVEDFAGSOPPGAVE
         KOMMENTARUTG
         KOMPENDIUM
         LEKSIKON
         LISENSIATAVH
         LÃ†REBOK
         MAGISTERAVH
         MASTERGRADSOPPG
         MONOGRAFI
         OPPSLAGSVERK
         OVERSETTELSE_BOK
         POPVIT_BOK
         RAPPORT
         UTSTILLINGSKAT
         """ .

:FAGFELT_Class
    a               rdfs:Class ;
    rdfs:subClassOf :CristinClass ;
    rdfs:comment    """The scientific field in which the book is published""" ;
    rdfs:subClassOf :TYPE_BOK_RAPPORT_Class .

:TYPE_TIDSSKRIFTPUBLIKASJON_Class
    a               rdfs:Class ;
    rdfs:subClassOf :CristinClass ;
    rdfs:comment    """
        A type of publication/result published in a journal, typically articles, reviews or editorials.
       """ .


:TIDSSKRIFT_Class
    a               rdfs:Class ;
    rdfs:subClassOf :CristinClass ;
    rdfs:comment    """A journal""" .

:VARBEID_EMNEORD_Class
    a               rdfs:Class ;
    rdfs:subClassOf :CristinClass ;
    rdfs:comment    """A keyword that is relative to a publication.""" .

:cristinfield
    a            rdf:Property ;
    rdfs:comment "Any property of any Cristin class" ;
    rdfs:domain  :CristinClass ;
    rdfs:range   rdfs:Class .


:mapstonvafield
    a           rdf:Property ;
    rdfs:range  xsd:string ;
    rdfs:domain :cristinfield .

:isignored
    a           rdf:Property ;
    rdfs:range  xsd:boolean ;
    rdfs:domain :cristinfield .

:id
    a               :cristinfield ;
    rdfs:comment    "Identifier of Cristin Result entry." ;
    rdfs:range      xsd:positiveInteger ;
    rdfs:domain     :Result ;
    :mapstonvafield """
        "additionalIdentifiers":[
            {
                "source":"Cristin",
                "value": ":id"
            }
        ]
    """ .

:arstall
    a               :cristinfield ;
    rdfs:comment    "The year a resource (result) was published." ;
    rdfs:range      xsd:positiveInteger ;
    rdfs:domain     :Result ;
    :mapstonvafield """
        entityDescription.date.year = :arstall;
        entityDescription.date.month = null;
        entityDescription.date.day = null;
    """ .

:dato_opprettet
    a               :cristinfield ;
    rdfs:comment    """
    When the domain is :Result, it is the date the resource was registered in Cristin or its predecessor.
    When the domain is :VITENSKAPELIGARBEID_LOKAL, it is the date the resource was registered in NVI.
    """ ;
    rdfs:range      xsd:date ;
    rdfs:domain     :Result, :VITENSKAPELIGARBEID_LOKAL_Class ;
    :mapstonvafield "createdDate when the domain is :Result" ;
    :isignored      "true" .


:varbeidhovedkatkode
    a               :cristinfield ;
    rdfs:comment    """
    The general category of the resource. A collection of "varbeidunderkatkode" .

""" ;
    rdfs:range      xsd:string ;
    rdfs:domain     :Result ;
    :mapstonvafield "practically not in use because :varbeidunderkatkode can specify the type of publication" .

:varbeidunderkatkode
    a               :cristinfield ;
    rdfs:comment    """
        The more specific category of the resource. No specific range available at the moment.
        Each varbeidunderkatkode belongs to only one varbeidhovedkatkode and therefore the value of this field is enough
        to deduct the exact type of the publication.
        The range of this property is found here:  https://api.cristin.no/v2/results/categories?lang=nb ,  en
        """ ;
    rdfs:range      xsd:string ;
    rdfs:domain     :Result ;
    :mapstonvafield """
       entityDescription.reference.publicationInstance
       implementedMappings:
         Anthology -> BookAnthology
         Monograph -> BookMonograph
         Rapport -> ReportResearch
         Kapittel -> ChapterArticle
         Popvit_Kapittel -> ChapterArticle
         Faglig_Kapittel -> ChapterArticle
         Artikkel_Fag -> JournalArticle
         Bokanmeldelse -> JournalReview
         Doktorgradsavhandling -> DegreePhd
    """ .

:eierkode_opprettet
    a            :cristinfield ;
    rdfs:comment """
        eierkode_opprettet and brukernavn_opprettet are the primary key for idenitfying which user created the entry. As a general rule a physical person
        can have many usernames (brukernavn) but only one eierkode. This holds even if a physical person moves from institution to institution
        and/or changes roles. Duplicates that violate this assumption are possible to occur but they are not expected to be the rule.
     """ ;
    rdfs:range   xsd:string ;
    rdfs:domain  :Result .


:brukernavn_opprettet
    a            :cristinfield ;
    rdfs:comment """
        When the domain is :Result, eierkode_opprettet and brukernavn_opprettet are the primary key for idenitfying which user created the entry. As a general rule a physical person
        can have many usernames (brukernavn) but only one eierkode. This holds even if a physical person moves from institution to institution
        and/or changes roles. Duplicates that violate this assumption are possible to occur but they are not expected to be the rule.

        When it is :VITENSKAPELIGARBEID_LOKAL_Class it is the user who created the NVI entry."
     """ ;
    rdfs:range   xsd:string ;
    rdfs:domain  :Result, :VITENSKAPELIGARBEID_LOKAL_Class ;
    :isignored   "true" .


:eierkode_siste_endring
    a            :cristinfield ;
    rdfs:comment "Similar to eierkode_opprettet but it indicates who made the last change." ;
    rdfs:range   xsd:string ;
    rdfs:domain  :Result ;
    :isignored   "true" .

:brukernavn_siste_endring
    a            :cristinfield ;
    rdfs:comment """
    When the domain is :Result the meaning is similar to brukernavn_opprettet but it indicates who made the last change.
    When the domain is :VITENSKAPELIGARBEID_LOKAL_Class  then it is the username of the user who updated the NVI entry.
     """ ;
    rdfs:range   xsd:string ;
    rdfs:domain  :Result, :VITENSKAPELIGARBEID_LOKAL_Class ;
    :isignored   "true" .

:dato_siste_endring
    a            :cristinfield ;
    rdfs:comment """
    When the domain is :Result, then the date of the last update of the registration.
    When the domain is :VITENSKAPELIGARBEID_LOKAL_Class then it is date the NVI entry was last updated
        """ ;
    rdfs:range   xsd:date ;
    rdfs:domain  :Result, :VITENSKAPELIGARBEID_LOKAL_Class ;
    :isignored   "true" .


:publiseringstatuskode
    a               :cristinfield ;
    rdfs:comment    """
                            The publication status of the referenced publication, i.e. whether the publication status of the publication itself in the publisher (e.g. Elsevier)
                            Possible values are: IN_PRESS", "PUBLISERT" (and "TEST").
                            """ ;
    rdfs:range      :PublicationStatus ;
    rdfs:domain     :Result ;
    :mapstonvafield "status = PUBLISHED (hardcoded)" .

:dato_utgitt
    a            :cristinfield ;
    rdfs:comment "Date the resource was published (e.g. through Elsevier or in OpenAccess Journal)." ;
    rdfs:range   xsd:date ;
    rdfs:domain  :Result ;
    :isignored   "true" .

:arstall_rapportert
    a            :cristinfield ;
    rdfs:comment "Year that the resource was included in an NVI report." ;
    rdfs:range   xsd:positiveInteger ;
    rdfs:domain  :Result ;
    :isignored   "true" .

:merknadtekst
    a            :cristinfield ;
    rdfs:comment "Free text for super-users to add comments when it comes to NVI approvals." ;
    rdfs:range   xsd:string ;
    rdfs:domain  :Result ;
    :isignored   "true" .

:merknadtekst_godkjenning
    a            :cristinfield ;
    rdfs:comment "Free text for super-users to add explanations/details on why the publication was approved or rejectedfor NVI reporting." ;
    rdfs:range   xsd:string ;
    rdfs:domain  :Result ;
    :isignored   "true" .

:kildekode
    a            :cristinfield ;
    rdfs:comment """
    The source (provider) the result was imported from, if any.
    Mostly superseded by the list of import references in table VARBEID_KILDE
    It is a string containing arbitrary codes such as "scopus" "norart", "BIBSYS" etc.
    """ ;
    rdfs:range   xsd:string ;
    rdfs:domain  :Result, :VARBEID_KILDE_Class ;
    :isignored   "true" .

:kildepostid
    a            :cristinfield ;
    rdfs:comment """
    The id of the record the result was imported from in the source system (e.g. the SCOPUS id if the result was imported from Scopus ) .

See varbeid.kildekode. Mostly superseded by VARBEID_KILDE. It contains only the identifier found in the source system and cannot be
     de-referenced.
    """ ;
    rdfs:range   xsd:string ;
    rdfs:domain  :Result ;
    :isignored   "true" .

:kildeid
    a            :cristinfield ;
    rdfs:domain  :VARBEID_KILDE_Class ;
    rdfs:range   xsd:string ;
    rdfs:comment """
        The id of the record from the source it was imported
( e.g SCOPUS or FORSKDOK. Overseeds :kildepostid.
    """ .


:pubidnr
    a            :cristinfield ;
    rdfs:comment """
    A reference to the record corresponding to this result in the PIA import database.
    PIA is a database that holds imports from Scopus.
    """ ;
    rdfs:range   xsd:positiveInteger ;
    rdfs:domain  :Result ;
    :isignored   "true" .

:VARBEID_SPRAK
    a               :cristinfield ;
    rdfs:comment    """
    A language that this work has been published in, the respective title, and the respective abstract
    and an indication whether it is the original language or a translation.
    """ ;
    rdfs:range      :VARBEID_SPRAK_Class ;
    rdfs:domain     :Result ;
    :mapstonvafield """
        entityDescription.mainTitle, entityDescription.language
    """ .

:sprakkode
    a               :cristinfield ;
    rdfs:comment    """
    The language of the title and the abstract included in the VARARBEID_SPRAK or the TIDSSKRIFT entry.
    The range is ISO 639-1.
    Possibly null or (xx) to represent (n/a)
    """ ;
    rdfs:range      xsd:string ;
    rdfs:domain     :VARBEID_SPRAK_Class, :TIDSSKRIFT_Class ;
    :mapstonvafield """
        entityDescription.language if VARBEID_SPRAK.status_original is "J"
    """ .

:tittletekst
    a               :cristinfield ;
    rdfs:comment    "The title in the VARARBEID_SPRAK entry. It is supposed to be in the language described by :sprakkode" ;
    rdfs:range      xsd:string ;
    rdfs:domain     :VARBEID_SPRAK_Class ;
    :mapstonvafield """
        entityDescription.mainTitle  if VARBEID_SPRAK.status_original is "J"
    """ .


:sammendragtekst
    a               :cristinfield ;
    rdfs:comment    "The abstract in the VARARBEID_SPRAK entry. It is supposed to be in the language described by :sprakkode" ;
    rdfs:range      xsd:string ;
    rdfs:domain     :VARBEID_SPRAK_Class ;
    :mapstonvafield """
            entityDescription.abstract  if VARBEID_SPRAK.status_original is "J"
        """ .

:status_original
    a            :cristinfield ;
    rdfs:comment """
    Indicator of whether the title in the respective VARBEID_SPRAK is the original title or not.
    Known possible values are 'J' ('true')
        , 'N' (false) and NULL (free to interpretation ) .

""" ;
    rdfs:range   xsd:string ;
    rdfs:domain  :VARBEID_SPRAK_Class ;
    :isignored   "false" .

:VITENSKAPELIGARBEID_LOKAL
    a            :cristinfield ;
    rdfs:comment "See description of domain class" ;
    rdfs:domain  :Result ;
    rdfs:range   :VITENSKAPELIGARBEID_LOKAL_Class ;
    :isignored   "true" .

:VARBEID_PERSON
    a               :cristinfield ;
    rdfs:comment    "A contributor to the respective result entry." ;
    rdfs:range      :VARBEID_PERSON_Class ;
    rdfs:domain     :Result ;
    :mapstonvafield "entityDescription.Contributor" .

:personlopenr
    a               :cristinfield ;
        rdfs:comment """
    It refers to a person's CristinId.
    When the domain is :VARBEID_PERSON_Class then it is a reference to a contributor.
    When the domain is "PRESENTASJON_VARBEID_Class and  the respective presentasjonstypekode is equal to "PERSON", tt refers to a contributor that has chosen
    to show this publication as one of their "important", "significant" etc publications.
    """;
    rdfs:range      xsd:positiveInteger ;
    rdfs:domain     :VARBEID_PERSON_Class , :PRESENTASJON_VARBEID_Class ;
    :mapstonvafield " when the domain is:VARBEID_PERSON_Class it maps entityDescription.contributor.identity.id" ;
    :isignored   false.


:fornavn
    a               :cristinfield ;
    rdfs:comment    """The first/given name of the contributor of the respective result entry.
                        This value is submitted manually by the user, in order to reflect what the user submitted as their first name when they
                        submitted the publication to the publisher
(e.g. Elsevier)
        """ ;
    rdfs:range      xsd:string ;
    rdfs:domain     :VARBEID_PERSON_Class ;
    :mapstonvafield "entityDescription.contributor.identity.fullanme" .

:etternavn
    a               :cristinfield ;
    rdfs:comment    """
    The surname/family-name of the contributor of the respective result entry
    This value is submitted manually by the user, in order to reflect what the user submitted as their first name when they
        submitted the publication to the publisher ( e.g. Elsevier ) .

""" ;
    rdfs:range      xsd:string ;
    rdfs:domain     :VARBEID_PERSON_Class ;
    :mapstonvafield "entityDescription.contributor.identity.fullanme" .

:VARBEID_PERSON_STED
    a               :cristinfield ;
    rdfs:comment    """
    Details about the institution which the contributor belongs to and the contributors role to the institution
    at the time the publication was registered in Cristin.
    """ ;
    rdfs:range      :VARBEID_PERSON_STED_Class ;
    rdfs:domain     :VARBEID_PERSON_Class ;
    :mapstonvafield "entityDescription.contributor.affiliation" .


:institusjonsnr
    a               :cristinfield ;
    rdfs:comment    """
    The **current** Cristin institution identifier institution that the contributor of the publication was affiliated with.
    This value may have changed from the time of entry was registered in
Cristin.
   :institusjonsnr
        ,   :avdnr, :undavdnr, and :gruppenr form a unique identifier of the Contributor's affiliation.

    """ ;
    rdfs:range      xsd:positiveInteger ;
    rdfs:domain     :VARBEID_PERSON_STED_Class ;
    :mapstonvafield "entityDescription.contributor.affiliation.id" .

:avdnr
    a               :cristinfield ;
    rdfs:comment    """
    The **current** Cristin Department number that the contributor of the publication was affiliated with at the time of creation of the
    registration entry.
    This value may have changed from the time of entry was registered in Cristin.
    See example in the definition of the domain class :VARBEID_PERSON_STED_Class
    """ ;
    rdfs:range      xsd:positiveInteger ;
    rdfs:domain     :VARBEID_PERSON_STED_Class ;
    :mapstonvafield "entityDescription.contributor.affiliation.id" .

:undavdnr
    a               :cristinfield ;
    rdfs:comment    """
    The current Sub-department number that the contributor of the publication was affiliated with at the time of creation of the
    registration entry.
    This value may have changed from the time of entry was registered in Cristin.
    See example in the definition of the domain class :VARBEID_PERSON_STED_Class
    """ ;
    rdfs:range      xsd:positiveInteger ;
    rdfs:domain     :VARBEID_PERSON_STED_Class ;
    :mapstonvafield "entityDescription.contributor.affiliation.id" .

:gruppenr
    a               :cristinfield ;
    rdfs:comment    """
     The current group number that the contributor of the publication was affiliated with at the time of creation of the registration entry.
     This value may have changed from the time of entry was registered in Cristin.
    """ ;
    rdfs:range      xsd:positiveInteger ;
    rdfs:domain     :VARBEID_PERSON_STED_Class ;
    :mapstonvafield "entityDescription.contributor.affiliation.id" .

:stedkode_opprinnelig
    a            :cristinfield ;
    rdfs:comment """
    This is a concatenation of :institusjonsnr, :avdnr, :undavdnr and gruppenr and it indicates the original identifier of the
    institution when the Cristin entry was created. This is an immutable value that never changes after its creation.
    """ ;
    rdfs:range   xsd:string ;
    rdfs:domain  :VARBEID_PERSON_STED_Class ;
    :isignored   "true" .

:institusjonsnavn_opprinnelig
    a            :cristinfield ;
    rdfs:comment "The original name of the institution at the time the Cristin entry was created. Immutable value" ;
    rdfs:range   xsd:string ;
    rdfs:domain  :VARBEID_PERSON_STED_Class ;
    :isignored   "true" .

:avdelingsnavn_opprinnelig
    a            :cristinfield ;
    rdfs:comment "The original name of the department at the time the Cristin entry was created. Immutable value" ;
    rdfs:range   xsd:string ;
    rdfs:domain  :VARBEID_PERSON_STED_Class ;
    :isignored   "true" .

:stednavn_opprinnelig
    a            :cristinfield ;
    rdfs:comment """
    The original name of the faculty/group that the Contributor was affiliated with at the time the Cristin entry was created.
    Hierarchically, this is the name of the lowest (most specific) entity that the Contributor is affiliated with.
     """ ;
    rdfs:range   xsd:string ;
    rdfs:domain  :VARBEID_PERSON_STED_Class ;
    :isignored   "true" .

:vekting
    a            :cristinfield ;
    rdfs:comment "SHOULD BE REMOVED FROM THE IMPORTS." ;
    rdfs:range   rdf:nil ; #unknown range
    rdfs:domain  :VARBEID_PERSON_STED_Class ;
    :isignored   "true" .

:VARBEID_PERSON_STED_ROLLE
    a               :cristinfield ;
    rdfs:comment    """
        The role of the respective Contributor for the respective publication affiliated for this role with the respective institution.
        This entry is immutable and does not change in time.
        """ ;
    rdfs:range      :VARBEID_PERSON_STED_ROLLE_Class ;
    rdfs:domain     :VARBEID_PERSON_STED_Class ;
    :mapstonvafield "entityDescription.contributor.role. only the first role of a person is considered." .

:rollekode
    a               :cristinfield ;
    rdfs:comment    """
        The role of the respective Contributor for the respective publication affiliated for this role with the respective institution.
        This entry is immutable and does not change in time.
        """ ;
    rdfs:range      xsd:string ;
    rdfs:domain     :VARBEID_PERSON_STED_ROLLE_Class ;
    :isignored      "false" ;
    :mapstonvafield " maps to NVA Role" .

:eierkode
    a            :cristinfield ;
    rdfs:range   xsd:string ;
    rdfs:domain  :VITENSKAPELIGARBEID_LOKAL_Class ;
    rdfs:comment """The institution the currently owns the NVI result. Example UIO.
    We do not know whether the values of this field are standardized and whether there is a defined set of values for this property's range""" ;
    :isignored   "true" .


:status_kontrollert
    a            :cristinfield ;
    rdfs:range   xsd:string ;
    rdfs:domain  :VITENSKAPELIGARBEID_LOKAL_Class ;
    rdfs:comment """
     It refers to the respective institution's opinion on whether the Cristin entry should be reported to NVI and count towards RBK funding.
    NULL = this institution has not yet given their opinion
    J = this institution believes the current result should be included in the NVI report
    N = this institution believes the current result should NOT be included in the NVI report (e.g. doesn't meet academic standards, or has other issues)
    """ ;
    :isignored   "true" .

:brukernavn_kontrollert
    a            :cristinfield ;
    rdfs:range   xsd:string ;
    rdfs:domain  :VITENSKAPELIGARBEID_LOKAL_Class ;
    rdfs:comment """
     The username who controlled / judged / validated the respective entry representing  their respective institution,
     indicated  by the field VITENSKAPELIGARBEID_LOKAL.eierkode.
    """ ;
    :isignored   "true" .

:dato_kontrollert
    a            :cristinfield ;
    rdfs:range   xsd:string ;
    rdfs:domain  :VITENSKAPELIGARBEID_LOKAL_Class ;
    rdfs:comment """
     The date the respective entry was controlled by the user defined by the fields (brukernavn_kontrollert, eierkode) in the object VITENSKAPELIGARBEID_LOKAL.
    """ ;
    :isignored   "true" .

:status_bekreftet_arkivsporsmal
    a            :cristinfield ;
    rdfs:range   xsd:string ;
    rdfs:domain  :VITENSKAPELIGARBEID_LOKAL_Class ;
    rdfs:comment """UNKNOWN meaning""" ;
    :isignored   "true" .

:brukernavn_avlvrt_arkivsystem
    a            :cristinfield ;
    rdfs:range   xsd:string ;
    rdfs:domain  :VITENSKAPELIGARBEID_LOKAL_Class ;
    rdfs:comment """UNKNOWN meaning""" ;
    :isignored   "true" .

:dato_avlvrt_arkivsystem
    a            :cristinfield ;
    rdfs:range   xsd:dateTimeStamp ;
    rdfs:domain  :VITENSKAPELIGARBEID_LOKAL_Class ;
    rdfs:comment """UNKNOWN meaning""" ;
    :isignored   "true" .

:status_fulgt_medf_reg
    a            :cristinfield ;
    rdfs:range   xsd:string ;
    rdfs:domain  :VITENSKAPELIGARBEID_LOKAL_Class ;
    rdfs:comment """UNKNOWN meaning""" ;
    :isignored   "true" .

:brukernavn_svart_medforf_reg
    a            :cristinfield ;
    rdfs:range   xsd:string ;
    rdfs:domain  :VITENSKAPELIGARBEID_LOKAL_Class ;
    rdfs:comment """UNKNOWN meaning""" ;
    :isignored   "true" .

:dato_svart_medforf_regel
    a            :cristinfield ;
    rdfs:range   xsd:string ;
    rdfs:domain  :VITENSKAPELIGARBEID_LOKAL_Class ;
    rdfs:comment """UNKNOWN meaning""" ;
    :isignored   "true" .



:TYPE_MEDIEBIDRAG
    a            :cristinfield ;
    rdfs:range   :TYPE_MEDIEBIDRAG_Class ;
    rdfs:domain  :Result ;
    rdfs:comment """A Cristin Result will have such a field only when its :varbeidunderkatkode has one of the following values:
	PROGLEDELSE, PROGDELTAGELSE, DOKUMENTAR, INTERVJU""" ;
    :isignored   true .

:varbeidlopenr
    a            :cristinfield ;
    rdfs:range   xsd:integer ;
    rdfs:domain  :TYPE_MEDIEBIDRAG_Class ;
    rdfs:comment """The Cristin Id of the respective :Result .

It is a self reference.""" ;
    :isignored   true .


:PRESENTASJON_VARBEID
    a            :cristinfield ;
    rdfs:range   :PRESENTASJON_VARBEID_Class ;
    rdfs:domain  :Result ;
    rdfs:comment """A project that the respective publication is part of.""" ;
    :isignored   false .

:presentasjonslopenr
    a            :cristinfield ;
    rdfs:range   xsd:integer ;
    rdfs:domain  :PRESENTASJON_VARBEID_Class ;
    rdfs:comment """ When the value of "presentasjonstypekode" is equal to :PRESENTASJONSTYPEKODE_PROSJEKT, it contains the project's Cristin ID.
    Otherwise its value has no meaning.
    """ ;
    :isignored   false .

:presentasjonstypekode
    a            :cristinfield ;
    rdfs:range   :PRESENTASJONSTYPEKODE_VALUES_Class ;
    rdfs:domain  :PRESENTASJON_VARBEID_Class ;
    rdfs:comment """
    When the value is equal to :PRESENTASJONSTYPEKODE_PROSJEKT, then it indicates that the respective PRESENTASJON_VARBEID_Class instance
    is a reference to a Cristin project.
    When the value is equal to :PRESENTASJONSTYPEKODE_PERSON, it indicates that it belongs to the collection of "important", "preferred"
    publications of the author.
    """ ;
    :isignored   false .



:TYPE_BOK_RAPPORT
    a               :cristinfield ;
    rdfs:range      :TYPE_BOK_RAPPORT_Class ;
    rdfs:domain     :Result ;
    :mapstonvafield """
        entityDescription.reference.publicationInstance.pages,
        entityDescription.reference.publicationContext.isbnList,
        entityDescription.reference.publicationContext.publisher
        entityDescription.npiSubjectHeading
    """ .

:antall_sider_totalt
    a               :cristinfield ;
    rdfs:comment    """
    The total number of pages.
    """ ;
    rdfs:range      xsd:positiveInteger ;
    rdfs:domain     :TYPE_BOK_RAPPORT_Class ;
    :mapstonvafield """
        entityDescription.reference.publicationInstance.pages
    """ .

:isbn
    a               :cristinfield ;
    rdfs:comment    "The isbn which the respective book is registered with. Is nullable when the domain is :TIDSSKRIFTSERIE_Class." ;
    rdfs:range      xsd:string ;
    rdfs:domain     :TYPE_BOK_RAPPORT_Class ;
    :mapstonvafield """
        entityDescription.reference.publicationContext.isbnList
    """ .

:utgivernavn
    a               :cristinfield ;
    rdfs:comment    "The name of the publisher of the respective book. Can be empty." ;
    rdfs:range      xsd:string ;
    rdfs:domain     :TYPE_BOK_RAPPORT_Class ;
    :mapstonvafield """
            entityDescription.reference.publicationContext.publisher
        """ .


:fagfelt
    a            :cristinfield ;
    rdfs:comment "The scientific field in which the book is published" ;
    rdfs:range   :FAGFELT_Class ;
    rdfs:domain  :TYPE_BOK_RAPPORT_Class ;
.


:fagfeltkode
    a               :cristinfield ;
    rdfs:comment    "The (numerical) code representing the scientific field in which the book is published" ;
    rdfs:range      xsd:positiveInteger ;
    rdfs:domain     :FAGFELT_Class ;
    :mapstonvafield """
            entityDescription.npiSubjectHeading
        """ .

:fagomradekode
    a            :cristinfield ;
    rdfs:comment "The (abriviation) code representing the scientific field in which the book is published" ;
    rdfs:range   xsd:string ;
    rdfs:domain  :FAGFELT_Class ;
    :isignored   "true" .

:navn
    a            :cristinfield ;
    rdfs:comment "The name of the scientific field in which the book is published" ;
    rdfs:range   xsd:string ;
    rdfs:domain  :FAGFELT_Class ;
    :isignored   "true" .

:navn_engelsk
    a            :cristinfield ;
    rdfs:comment "The english name of the scientific field in which the book is published" ;
    rdfs:range   xsd:string ;
    rdfs:domain  :FAGFELT_Class ;
    :isignored   "true" .

:TYPE_TIDSSKRIFTPUBLIKASJON
    a               :cristinfield ;
    rdfs:comment    """
    A type publication called tidsskrift.
    """ ;
    rdfs:range      :TYPE_TIDSSKRIFTPUBLIKASJON_Class ;
    rdfs:domain     :Result ;
    :mapstonvafield """
        entityDescription.reference.publicationInstance.volume,
        entityDescription.reference.publicationInstance.pages.begin,
        entityDescription.reference.publicationInstance.pages.end,
        entityDescription.reference.doi
    """ .

:volum
    a               :cristinfield ;
    rdfs:comment    """
    The volume in which the article is published. The value is a number in the form of a string. Possibly null.
    """ ;
    rdfs:range      xsd:string ;
    rdfs:domain     :TYPE_TIDSSKRIFTPUBLIKASJON_Class ;
    :mapstonvafield """
        entityDescription.reference.publicationInstance.volume
    """ .

:sidenr_fra
    a               :cristinfield ;
    rdfs:comment    "The page number the that marks the start of the article. The value is a number in the form of a string. Possibly null." ;
    rdfs:range      xsd:string ;
    rdfs:domain     :TYPE_TIDSSKRIFTPUBLIKASJON_Class ;
    :mapstonvafield """
        entityDescription.reference.publicationInstance.pages.begin
    """ .

:sidenr_til
    a               :cristinfield ;
    rdfs:comment    "The page number the that marks the end of the article. The value is a number in the form of a string. Possibly null." ;
    rdfs:range      xsd:string ;
    rdfs:domain     :TYPE_TIDSSKRIFTPUBLIKASJON_Class ;
    :mapstonvafield """
        entityDescription.reference.publicationInstance.pages.end
    """ .

:doi
    a               :cristinfield ;
    rdfs:comment    "The doi connected to the respective article. Possibly null." ;
    rdfs:range      xsd:string ;
    rdfs:domain     :TYPE_TIDSSKRIFTPUBLIKASJON_Class ;
    :mapstonvafield """
        entityDescription.reference.doi
    """ .

:antall_sider_totalt
    a               :cristinfield ;
    rdfs:comment    "The total number of pages. Possibly null." ;
    rdfs:range      rdf:nil ; #unknown range
    rdfs:domain     :TYPE_TIDSSKRIFTPUBLIKASJON_Class ;
    :isignored   "true" .

:publiseringsar
    a               :cristinfield ;
    rdfs:comment    "The year of publication for the journal" ;
    rdfs:range      xsd:positiveInteger ;
    rdfs:domain     :TYPE_TIDSSKRIFTPUBLIKASJON_Class ;
    :isignored   "true" .

:hefte
    a               :cristinfield ;
    rdfs:comment    "The booklet containing the publication. Data in the form of a number stored as a string" ;
    rdfs:range      xsd:string ;
    rdfs:domain     :TYPE_TIDSSKRIFTPUBLIKASJON_Class ;
    :isignored   "true" .

:status_referee_ordning
    a               :cristinfield ;
    rdfs:comment    "Defines whether or not the Journal is peerreviewed (J)=yes, (N)=no and NULL." ;
    rdfs:range      xsd:string ;
    rdfs:domain     :TYPE_TIDSSKRIFTPUBLIKASJON_Class ;
    :isignored   "true" .

:supplement
    a               :cristinfield ;
    rdfs:comment    "A area for adding information about possible attachments to the article." ;
    rdfs:range      xsd:string ;
    rdfs:domain     :TYPE_TIDSSKRIFTPUBLIKASJON_Class ;
    :isignored   "true" .

:utbredelsesomrade
    a               :cristinfield ;
    rdfs:comment    """
        Information about where or to what extent the article has been published.
        Examples: NORSK, NORDISK, INTERNASJ, NASJONALT, UKJENT""" ;
    rdfs:range      xsd:string ;
    rdfs:domain     :TYPE_TIDSSKRIFTPUBLIKASJON_Class ;
    :isignored   "true" .

:artikkelnummer
    a               :cristinfield ;
    rdfs:comment    """
        A number identifying the article within the journal.
        This might be a sequence number or the actuall ID of the article, this is decided by the journal
        The ID consists of a combination of letters and numbers or just numbers.
        Examples: L08802, 1588, 2.
        Possibly null.
        """ ;
    rdfs:range      xsd:string ;
    rdfs:domain     :TYPE_TIDSSKRIFTPUBLIKASJON_Class ;
    :isignored   "true" .

:arstall_trykket
    a               :cristinfield ;
    rdfs:comment    "The year the publication was printed." ;
    rdfs:range      xsd:positiveInteger ;
    rdfs:domain     :TYPE_TIDSSKRIFTPUBLIKASJON_Class ;
    :isignored   "true" .

:arstall_online
    a               :cristinfield ;
    rdfs:comment    "The year the publication was released online." ;
    rdfs:range      xsd:positiveInteger ;
    rdfs:domain     :TYPE_TIDSSKRIFTPUBLIKASJON_Class ;
    :isignored   "true" .

:TIDSSKRIFT
    a               :cristinfield ;
    rdfs:comment    """
    A journal, in this case the journal in which the publication was published.
    """ ;
    rdfs:range      :TIDSSKRIFT_Class ;
    rdfs:domain     :TYPE_TIDSSKRIFTPUBLIKASJON_Class ;
    :mapstonvafield """
        entityDescription.reference.publicationContext.printIssn
    """ .

:issn
    a               :cristinfield ;
    rdfs:comment    "The issn connected to the respective article. Possibly null." ;
    rdfs:range      xsd:string ;
    rdfs:domain     :TIDSSKRIFT_Class ;
    :mapstonvafield """
        entityDescription.reference.publicationContext.printIssn
    """ .

:issn_elektronisk
    a               :cristinfield ;
    rdfs:comment    "The online version of the issn connected to the respective article. Possibly null." ;
    rdfs:range      xsd:string ;
    rdfs:domain     :TIDSSKRIFT_Class ;
    :mapstonvafield """
        entityDescription.reference.publicationContext.onlineIssn
    """ .

:tidsskriftnavn
    a               :cristinfield ;
    rdfs:comment    "The name of the journal publishing the article" ;
    rdfs:range      xsd:string ;
    rdfs:domain     :TIDSSKRIFT_Class ;
    :mapstonvafield """
        entityDescription.reference.publicationContext.title
    """ .

:tidsskriftnr
    a               :cristinfield ;
    rdfs:comment    "Number identifying the specific journal within Cristin" ;
    rdfs:range      xsd:positiveInteger ;
    rdfs:domain     :TIDSSKRIFT_Class ;
    :isignored   "true" .

:nsdkode
    a               :cristinfield ;
    rdfs:comment    "A code representing the id in NSD-channelregistry " ;
    rdfs:range      rdf:nil ; #unknown range
    rdfs:domain     :TIDSSKRIFT_Class ;
    :isignored   "true" .

:landkode_utgiver
    a               :cristinfield ;
    rdfs:comment    """
        The code identifying the country where the publisher is located.
        Example: NO
        Possibly null.""" ;
    rdfs:range      xsd:string ;
    rdfs:domain     :TIDSSKRIFT_Class ;
    :isignored   "true" .

:status_referee_ordning
    a               :cristinfield ;
    rdfs:comment    "Defines whether or not the Journal is peerreviewed (J)=yes, (N)=no, (U)=uncertain and NULL." ;
    rdfs:range      xsd:string ;
    rdfs:domain     :TIDSSKRIFT_Class ;
    :isignored   "true" .

:dato_utgatt
    a               :cristinfield ;
    rdfs:comment    """If the journal no longer exists this is the date when it disapeared.
    Information about what if any: replaced it, it merged into, or what it developed into.
    Info can be found with NSD and Cristin but is not exported as of today.
    """ ;
    rdfs:range      xsd:string ;
    rdfs:domain     :TIDSSKRIFT_Class ;
    :isignored   "true" .

:status_serie
    a               :cristinfield ;
    rdfs:comment    """Defines wheter it is a bookseries or not (in that case a Journal).
    (J) declares it to be a bookseries something we dont want/expect to find here""" ;
    rdfs:range      xsd:string ;
    rdfs:domain     :TIDSSKRIFT_Class ;
    :isignored   "true" .

:VARBEID_EMNEORD
    a               :cristinfield ;
    rdfs:comment    """ See the range class.""" ;
    rdfs:range      :VARBEID_EMNEORD_Class ;
    rdfs:domain     :Result ;
    :mapstonvafield """
        entityDescription.tags,
    """ .

:emneordnavn_bokmal
    a               :cristinfield ;
    rdfs:comment    """
    The bokmal version of the VARBEID_EMNEORD. Possibly null.
    """ ;
    rdfs:range      xsd:string ;
    rdfs:domain     :VARBEID_EMNEORD_Class ;
    :mapstonvafield """
        entityDescription.tags
    """ .

:emneordnavn_engelsk
    a               :cristinfield ;
    rdfs:comment    "The english version of the VARBEID_EMNEORD. Possibly null." ;
    rdfs:range      xsd:string ;
    rdfs:domain     :VARBEID_EMNEORD_Class ;
    :mapstonvafield """
        entityDescription.tags
    """ .

:emneordnavn_nynorsk
    a               :cristinfield ;
    rdfs:comment    "The nynorsk version of the the VARBEID_EMNEORD. Possibly null." ;
    rdfs:range      xsd:string ;
    rdfs:domain     :VARBEID_EMNEORD_Class ;
    :mapstonvafield """
        entityDescription.tags
        """ .

:emneordlopenr
    a            :cristinfield ;
    rdfs:comment "The Cristin ID of the keyword (emneord)" ;
    rdfs:range   xsd:integer  ;
    rdfs:domain  :VARBEID_EMNEORD_Class ;
    :isignored   "true" .
